%%%%%%%%%%%%%%%%%%%%%%%%%%%%%%%%%%%%%%%%%%%%%%%%%%%%%%%%%%%%%%%%%%%%%%%%%%%%%%%%%%%%%%%%%%%%%%%%%%%%%%%%%%%%%%%%%%%%%%%%%%%%%%%%%%%%%%%%%%%%%%%%%%%%%%%%%%%%%%%%%%%
% Written By Michael Brodskiy
% Class: Fundamentals of Linear Systems
% Professor: I. Salama
%%%%%%%%%%%%%%%%%%%%%%%%%%%%%%%%%%%%%%%%%%%%%%%%%%%%%%%%%%%%%%%%%%%%%%%%%%%%%%%%%%%%%%%%%%%%%%%%%%%%%%%%%%%%%%%%%%%%%%%%%%%%%%%%%%%%%%%%%%%%%%%%%%%%%%%%%%%%%%%%%%%

\include{Includes.tex}

\title{Homework 8}
\date{\today}
\author{Michael Brodskiy\\ \small Professor: I. Salama}

\begin{document}

\maketitle

\begin{enumerate}

  \item

    \begin{enumerate}

      \item By the duality property, we may write:

        $$\cos(\omega_o t)\leftrightarrow \pi\left[ \delta(\omega-\omega_o)+\delta(\omega+\omega_o) \right]$$
        $$\pi\left[ \delta(t-t_o)+\delta(t+t_o) \right]\leftrightarrow 2\pi\cos(\omega t_o)$$

        In tandem with the time shifting property, we may write:

        $$\frac{1}{2}e^{-\alpha j\omega}\left[ \delta(t-t_o)+\delta(t+t_o) \right]\leftrightarrow \cos(\omega t_o-\alpha)$$

        This gives us:

        $$\boxed{x(t)=\frac{1}{2}e^{-\frac{\pi j \omega}{3}}\left[ \delta(t-4)+\delta(t+4) \right]}$$

      \item We may use the following known transform formulas:

        $$\pi\left[ \delta(\omega-\omega_o)+\delta(\omega+\omega_o) \right]\leftrightarrow \cos(\omega_o t)$$
        $$\frac{\pi}{j}\left[ \delta(\omega-\omega_o)-\delta(\omega+\omega_o) \right]\leftrightarrow \sin(\omega_o t)$$
        $$\frac{1}{(\alpha+j\omega)^2}\leftrightarrow te^{-\alpha t}u(t)$$

        In combination with the time shifting property, we may get:

        $$\boxed{x(t)=\frac{2}{\pi}\cos(5t-3)-4j\pi\sin(2\pi t)+te^{-2t}u(t)}$$

    \end{enumerate}

  \item

    \begin{enumerate}

      \item The signal $x(t)$ may be expressed in several parts: a step up by 1 at $t=-1$ to $t=1$, a slope of 1 between $-1$ and $1$, and a step up of $2$ for $t>1$. Thus, we get:

        $$\boxed{x(t)=r(t+1)-r(t-1)}$$

        This lets us find:

        $$\boxed{\frac{dx}{dt}=u(t+1)-u(t-1)}$$

        And finally:

        $$\boxed{\frac{d^2x}{dt^2}=\delta(t+1)-\delta(t-1)}$$

      \item The DC component can be accounted for using:

        $$x_{DC}=\lim_{T\to\infty}\frac{1}{T}\int_{-\frac{T}{2}}^{\frac{T}{2}} x(t)\,dt$$

        This gives:

        $$x_{DC}=\lim_{T\to\infty} \frac{1}{T}\left[ \int_{-1}^{1}(t+1)\,dt+\int_1^{\frac{T}{2}} 2\,dt \right]$$
        $$x_{DC}=\lim_{T\to\infty} \frac{1}{T}\left[ 2+2\left( \frac{T}{2}-1 \right) \right]$$
        $$x_{DC}=1$$

        Using the duality property, we may write:

        $$1\leftrightarrow 2\pi\delta(\omega)$$

        We then transform the second order derivative to see:

        $$\mathcal{F}\left\{ \frac{d^2x(t)}{dt^2} \right\}=e^{j\omega} -e^{-j\omega}$$
        $$(j\omega)^2X(\omega)=e^{j\omega} -e^{-j\omega}$$

        This gives us:

        $$X(j\omega)=-\frac{2j\sin(\omega)}{\omega^2}$$
          
        We then add in the DC component to get:

        $$\boxed{X(j\omega)=2\pi\delta(\omega)-\frac{2j\sin(\omega)}{\omega^2}}$$

      \item Given that the subtraction of the 1 removes the DC component, we simply get:

        $$\boxed{G(j\omega)=-\frac{2j\sin(\omega)}{\omega^2}}$$

    \end{enumerate}

    \setcounter{enumi}{3}

  \item

    \begin{enumerate}

      \item Per the theorem, we may write:

        $$\int_{-\infty}^{\infty}|x(t)|^2=\frac{1}{2\pi}\int_{-\infty}^{\infty} |X(\omega)|^2\,d\omega$$
        $$2\pi\int_{-\infty}^{\infty}|x(t)|^2=\int_{-\infty}^{\infty} |X(\omega)|^2\,d\omega$$

        This allows us to write:

        $$A=4\pi\int_{0}^{\infty}e^{-4t}\,dt$$
        $$-\pi \left(e^{-4t}\right)\Big|_0^{\infty}$$
        $$-\pi \left(e^{-4\infty}-1\right)$$

        Thus, we obtain:

        $$\boxed{A=\pi}$$

      \item Per our Fourier transform properties, we may write:

        $$tx(t)\to j\frac{d}{d\omega}X(\omega)$$

        For $y(t)=te^{-2|t|}$ this gives us:

        $$Y(j\omega)=j\frac{d}{d\omega}\left[ \frac{4}{(4+\omega^2)} \right]$$

        Differentiating gives us the final answer as:

        $$\boxed{Y(j\omega)=-\frac{8j\omega}{(4+\omega^2)^2}}$$

      \item By the duality property, we know that if $x(t)\leftrightarrow X(j\omega)$, then:

        $$x(t)\leftrightarrow 2\pi X(-j\omega)$$

        As such, we may write:

        $$-\frac{8jt}{(4+t^2)^2}\leftrightarrow 2\pi(-\omega)e^{-2|\omega|}$$
        $$\frac{t}{(4+t^2)^2}\leftrightarrow -j\pi\omega e^{-2|\omega|}$$

        Thus, we see that:

        $$\boxed{\mathcal{F}\left\{ \frac{4t}{(4+t^2)^2} \right\}=-j\pi\omega e^{-2|\omega|}}$$

    \end{enumerate}

  \item We may compute the response of the system using the convolution; the convolution may be more easily computed using the Fourier transform such that:

    $$y(t)=h(t)*x(t)\leftrightarrow Y(j\omega)=H(j\omega)X(j\omega)$$

    We can see that the given response may be written as:

    $$H(j\omega)=\left\{\begin{array}{ll} e^{-3j\omega},&|\omega|\leq4\\0,&\text{otherwise}\end{array}$$

    \begin{enumerate}

      \item We may see that the transform becomes:

        $$X_1(j\omega)=\pi e^{N\pi j\omega}\left[ \delta(\omega-10)+\delta(\omega+10) \right]$$

        We may observe that the response and signal do not have common values for which they are non-zero. This gives us:

        $$Y_1(j\omega)=0$$

        This ultimately means:

        $$\boxed{y_1(t)=0}$$

      \item We may see that the transform becomes:

        $$X_2(j\omega)=5\pi\left[ \delta(\omega-2)+\delta(\omega+2) \right]$$

        We multiply the two together to get:

        $$Y_2(j\omega)=5\pi e^{-3j\omega}\left[  \delta(\omega-2)+\delta(\omega+2)\right]$$

        We see this introduces a delay of three units, which gives us:

        $$\boxed{y_2(t)=5\cos(2(t-3))}$$

      \item We may see that the transform becomes:

        $$X_3(j\omega)=\left\{\begin{array}{ll} 1,&|\omega|\leq1\\0,&\text{otherwise}\end{array}$$

          Multiplying the two together creates a delayed sink function, but with the boundaries of the input:

        $$Y_3(j\omega)=\left\{\begin{array}{ll} e^{-3j\omega},&|\omega|\leq1\\0,&\text{otherwise}\end{array}$$

          Transforming back, we get:

          $$\boxed{y_3(t)=\frac{\sin(t-3)}{\pi(t-3)}}$$

        \item We may observe that the input signals within the passband of the filter simply introduce a delay at the output, thus, we may conclude:

          $$\boxed{y_4(t)=\left( \frac{\sin(t-3)}{\pi(t-3)} \right)^2}$$

    \end{enumerate}

  \item

    \begin{enumerate}

      \item We may apply the Laplace transform to get:

        $$s^2Y(s)+5sY(s)+4Y(s)=3X(s)$$

        Since we know that the response is the output over input, we may write:

        $$H(s)=\frac{3}{s^2+5s+4}$$
        $$H(s)=\frac{3}{(s+4)(s+1)}$$

        We use partial fraction decomposition in order to be able to apply the reverse transform. This gets us:

        $$H(s)=-\frac{1}{s+1}+\frac{1}{s+4}$$

        We take the inverse transform to conclude:

        $$\boxed{h(t)=[-e^{-t}+e^{-4t}]u(t)}$$

      \item Given the input $x(t)$, we may write:

        $$X(s)=\frac{1}{s+1}$$

        We know the response may be written as:

        $$Y(s)=H(s)X(s)$$

        And so we get:

        $$Y(s)=\frac{3}{(s+4)(s+1)^2}$$

        We once again use partial fraction decomposition to write:

        $$Y(s)=\frac{A}{s+1}+\frac{B}{(s+1)^2}+\frac{C}{s+4}$$
        $$Y(s)=\frac{-1}{3(s+1)}+\frac{1}{(s+1)^2}+\frac{1}{3(s+4)}$$

        We take the inverse transform to get:

        $$\boxed{y(t)=\left[-\frac{1}{3}e^{-t}+\frac{1}{3}e^{-4t}+te^{-t}\right]u(t)}$$

    \end{enumerate}

    \setcounter{enumi}{7}

  \item

    \begin{enumerate}

      \item We may take the Laplace transform of both to get:

        $$X(s)=\frac{1}{s+1}+\frac{2}{s+4}$$
        $$Y(s)=\frac{3}{s+1}-\frac{3}{s+3}$$

        We may combine the fractions to get:

        $$X(s)=\frac{3s+6}{(s+1)(s+4)}$$
        $$Y(s)=\frac{6}{(s+1)(s+3)}$$
        
        We know the response may be written as:

        $$H(s)=\frac{Y(s)}{X(s)}$$

        This gives us:

        $$H(s)=\frac{6}{(s+1)(s+3)}\cdot\frac{(s+1)(s+4)}{3s+6}$$
        $$H(s)=\frac{2s+8}{(s+2)(s+3)}$$

        Given that $s=j\omega$, we may write:

        $$H(j\omega)=\frac{2j\omega+8}{(j\omega+2)(j\omega+3)}$$

        We may simplify to get:

        $$\boxed{H(j\omega)=\frac{2j\omega+8}{6+5j\omega-\omega^2}}$$

      \item Using partial fraction decomposition, we may write:

        $$H(s)=\frac{A}{s+2}+\frac{B}{s+3}$$

        We may find that $A=4$ and $B=-2$ to get:

        $$H(s)=\frac{4}{s+2}-\frac{2}{s+3}$$

        Taking the inverse transform, we find:

        $$\boxed{h(t)=[4e^{-2t}-2e^{-3t}]u(t)}$$

      \item From part (a), we know:

        $$\frac{Y(s)}{X(s)}=\frac{2s+8}{(s+2)(s+3)}$$
        $$Y(s)[s^2+5s+6]=X(s)[2s+8]$$

        Taking the inverse transform, we get:

        $$\boxed{\frac{d^2y(t)}{dt}+5\frac{dy(t)}{dt}+6y(t)=2\frac{dx(t)}{dt}+8x(t)}$$

      \item For an inverse system, we know:

        $$H(s)H_i(s)=1$$

        As such, we get:

        $$H_i(s)=\frac{(s+2)(s+3)}{2s+8}$$

        Taking $s\to j\omega$, we get:

        $$\boxed{H_i(j\omega)=\frac{(j\omega+2)(j\omega+3)}{2j\omega+8}}$$

    \end{enumerate}

  \item To plot the signals, we may begin by converting them to their Fourier form. Moving in order, we may begin with $v_1(t)$ to observe:

    $$v_1(t)=x(t)\cdot2\cos(\omega_c t)$$
    $$V_1(j\omega)=2\pi\delta(\omega-\omega_c)+\delta(\omega+\omega-c)X(j\omega)$$

    Since, at $\omega_c$, $X(j\omega)=.5$, This gives us:

    \begin{figure}[H]
      \centering
      \include{Figures/HW8-9a}
      \caption{Spectrum of $V_1(j\omega)$}
      \label{fig:1}
    \end{figure}

    As a result of the filter, we may see that:
    
    $$W_1(j\omega)=2\pi\left[ \delta(\omega-\omega_c)+\delta(\omega-\omega_c) \right]$$

    Changing $\omega_c$ to $\omega_o$ per the given relationship, we get:

    \begin{figure}[H]
      \centering
      \include{Figures/HW8-9b}
      \caption{Spectrum of $W_1(j\omega)$}
      \label{fig:2}
    \end{figure}

    We then check $V_2(j\omega)$ to see that, because of the flipped sign in the transform of the $\sin$ term, the negative corner frequency has negative magnitude:

    \begin{figure}[H]
      \centering
      \include{Figures/HW8-9c}
      \caption{Spectrum of $V_2(j\omega)$}
      \label{fig:3}
    \end{figure}

    Because of the filter, however, we see that the spectrum of $W_2(j\omega)$ remains the same as that of $W_1(j\omega)$:

    \begin{figure}[H]
      \centering
      \include{Figures/HW8-9d}
      \caption{Spectrum of $W_2(j\omega)$}
      \label{fig:4}
    \end{figure}

    We see that combining the signals $W_{1,2}$ with the sinusoids results in Fourier responses consisting of rect functions, centered at $\pm\omega_c$, with a width of $2\omega_o$:

    \begin{figure}[H]
      \centering
      \include{Figures/HW8-9e}
      \caption{Spectrum of $Z_1(j\omega)$}
      \label{fig:5}
    \end{figure}

    \begin{figure}[H]
      \centering
      \include{Figures/HW8-9f}
      \caption{Spectrum of $Z_2(j\omega)$}
      \label{fig:6}
    \end{figure}

    Summing the signals gives us a height of 1, which indicates that this is a bandpass filter with center frequency $\omega_c$ and bandwidth $2\omega_o$:

    \begin{figure}[H]
      \centering
      \include{Figures/HW8-9g}
      \caption{Spectrum of $Y(j\omega)$}
      \label{fig:7}
    \end{figure}

  \item We may write the equivalent impedances of all of the components as:

    $$Z_L=.5s\quad\text{ and }Z_C=\frac{1}{2s}$$

    The equivalent impedance becomes:

    $$Z_{eq}=.5s+1+\frac{1}{2s}$$

    The current becomes:

    $$I(s)=\frac{X(s)}{Z_{eq}}$$

    Which means that the voltage across the capacitor, $y(t)$ is:

    $$Y(s)=\frac{\frac{1}{2s}X(s)}{.5s+1+\frac{1}{2s}}$$

    Since the response is output over input, we get:

    $$H(s)=\frac{1}{s^2+2s+1}$$
    $$H(s)=\frac{1}{(s+1)^2}$$

    This gives us the final response as:

    $$\boxed{h(t)=te^{-t}u(t)}$$

\end{enumerate}

\end{document}

