%%%%%%%%%%%%%%%%%%%%%%%%%%%%%%%%%%%%%%%%%%%%%%%%%%%%%%%%%%%%%%%%%%%%%%%%%%%%%%%%%%%%%%%%%%%%%%%%%%%%%%%%%%%%%%%%%%%%%%%%%%%%%%%%%%%%%%%%%%%%%%%%%%%%%%%%%%%%%%%%%%%
% Written By Michael Brodskiy
% Class: Fundamentals of Linear Systems
% Professor: I. Salama
%%%%%%%%%%%%%%%%%%%%%%%%%%%%%%%%%%%%%%%%%%%%%%%%%%%%%%%%%%%%%%%%%%%%%%%%%%%%%%%%%%%%%%%%%%%%%%%%%%%%%%%%%%%%%%%%%%%%%%%%%%%%%%%%%%%%%%%%%%%%%%%%%%%%%%%%%%%%%%%%%%%

\include{Includes.tex}

\title{Homework 6}
\date{\today}
\author{Michael Brodskiy\\ \small Professor: I. Salama}

\begin{document}

\maketitle

\begin{enumerate}

  \item

    \begin{enumerate}

      \item Per the rules of Laplace Transforms, we can convolve two signals by the rule that:

        $$y(t)=x_1(t)*x_2(t)\to Y(s)=X_1(s)X_2(s)$$

        As such, we may obtain:

        $$X_1(s)=\frac{1}{s+4}\quad\text{ and }\quad X_2(s)=\frac{1}{s+2}$$

        Now, we account for the shifts. We know that, for $x(t)\to x(t-t_o)$ the transform becomes $X(s)\to e^{st_o}X(s)$. Furthermore, we know that for $x(-t)\to X(-s)$. Thus, we find:

        $$X_1(s)=\frac{e^{-3s}}{-s+4}\quad\text{ and }\quad X_2(s)=\frac{e^{-2s}}{s+2}$$

        Multiplying together, we find:

        $$\boxed{Y(s)=\frac{e^{-5s}}{(4-s)(s+2)},\quad\text{ROC: } -2<\sigma<4}$$

      \item We may write this integral as the convolution of two functions:

        $$x_1(t)=\cos(2t)e^{-2t}$$
        $$x_2(t)=u(-3t+1)$$

        We now work to use the multiplicative property of the Laplace transform:

        $$\mathcal{L}\left\{ x_1(t) \right\}=\frac{s+2}{(s+2)^2+4}$$
        $$\mathcal{L}\left\{ x_2(t) \right\}=\frac{e^{-\frac{1}{3}s}}{s}$$

        We multiply the two together to get:

        $$\boxed{Y(s)=\frac{(s+2)e^{-\frac{1}{3}s}}{(s)[(s+2)^2+4]}}$$

        Note that we may also use the last property of Laplace transforms on our equation sheet to write:

        $$\int_t^{\infty} x(\tau)\,d\tau= \frac{1}{s}X(s)$$

        This gives us the same result:

        $$\boxed{Y(s)=\frac{(s+2)e^{-\frac{1}{3}s}}{(s)[(s+2)^2+4]}}$$

    \end{enumerate}

  \item

    First, we know that the poles must be at plus or minus the imaginary value, so the two poles must be at $s=-1\pm 3j$. Thus, we see that $X(s)$ can be expressed as:

    $$X(s)=\frac{k}{(s+1-3j)(s+1+3j)}$$
    $$X(s)=\frac{k}{(s+1)^2+3^2}$$

    We then apply the condition given in statement (5) to get:

    $$2=\frac{k}{(1^2)+(3^2)}$$
    $$k=20$$

    Then, because of statement (4), we know that $s=4$ is NOT in the ROC of $X(s)$. This means that we obtain the transform as:

    $$\boxed{X(s)=\frac{20}{(s+1)^2+3^2},\quad\text{ROC: }\sigma <-1}$$

    Taking the inverse transform, per our Laplace tables, we see:

    $$\boxed{x(t)=-\frac{20}{3}e^{-t}\sin(3t)u(-t)}$$

  \item

    \begin{enumerate}

      \item 

        Using our tables, we may obtain (with $X(s)$ ROC: $\sigma <3$ and $H(s)$ ROC: $\sigma>-2$):

        $$\boxed{X(s)=-\frac{5}{s-3}\quad\text{ and }H(s)=\frac{1}{s+2}}$$

      \item 

        We may write the convolution transform as:

        $$Y(s)=X(s)H(s)$$

        Thus, we get:

        $$Y(s)=\left( -\frac{5}{s-3} \right)\left( \frac{1}{s+2} \right)$$
        $$\boxed{Y(s)=-\frac{5}{(s-3)(s+2)}}$$

      \item 

        We begin by using partial fraction decomposition, which gives us:

        $$Y(s)=\frac{A}{s-3}+\frac{B}{s+2}$$

        From here, we get $A=-1$ and $B=1$, which gives us:

        $$Y(s)=\frac{-1}{s-3}+\frac{1}{s+2}$$

        Using our inverse transforms, we obtain:

        $$\boxed{y(t)=e^{3t}u(-t)+e^{-2t}u(t)}$$

      \item 

        Explicit convolution gives us:

        $$x(t)*h(t)=\int_0^t 5e^{3\tau}u(-\tau)e^{-2(t-\tau)}u(t-\tau)\,d\tau$$
        $$x(t)*h(t)=\int_0^t 5e^{-2t+5\tau}u(-\tau)u(t-\tau)\,d\tau$$

        We see that the function is bounded by:

        $$\tau \leq 0\quad\text{ and }\quad \tau\leq t$$

        From this, we may write:

        $$y(t)=-5e^t\int_0^t e^{5\tau}\,d\tau$$
        $$y(t)=-e^{-2t}\left[ e^{5\tau} \right]\Big|_0^t$$
        $$y(t)=-e^{-2t}\left[ e^{5t}-1 \right]$$

        This confirms:

        $$\boxed{y(t)=e^{3t}u(-t)+e^{-2t}u(t)}$$

    \end{enumerate}

  \item

    \begin{enumerate}

      \item 

        Taking the Laplace transform, we get:

        $$s^2Y(s)-sY(s)-6Y(s)=sX(s)$$
        $$Y(s)[s^2-s-6]=sX(s)$$
        $$\boxed{H(s)=\frac{Y(s)}{X(s)}=\frac{s}{s^2-s-6}}$$

        Thus, we see that there is a zero at $s=0$ and poles at $s=-2,3$. This allows us to plot:

        \begin{figure}[H]
          \centering
          \include{Figures/HW6-4a}
          \caption{Pole-Zero Plot}
          \label{fig:1}
        \end{figure}
        
      \item 

        We may begin by using partial fraction decomposition:

        $$\frac{s}{s^2-s-6}\Rightarrow \frac{A}{s-3}+\frac{B}{s+2}$$

        Plugging in our values, we find $A=3/5$ and $B=2/5$, which gives us:

        $$H(s)=\frac{3/5}{s-3}+\frac{2/5}{s+2}$$

        \begin{enumerate}

          \item When the system is stable, we know that the ROC must be bounded. Thus, we know that the ROC is $-2<\sigma<3$. Using our transform table, this gives:

            $$\boxed{h(t)=-\frac{3}{5}e^{3t}u(-t)+\frac{2}{5}e^{-2t}u(t)}$$

          \item When the system is causal, we know that the ROC is right-sided, such that $\sigma>3$. Thus, we see:

            $$\boxed{h(t)=\frac{3}{5}e^{3t}u(t)+\frac{2}{5}e^{-2t}u(t)}$$

          \item When it is neither stable nor causal, the ROC must be left-sided and can not include the j$\omega$ axis. This gives us:

            $$\boxed{h(t)=\frac{3}{5}e^{3t}u(t)-\frac{2}{5}e^{-2t}u(-t)}$$

        \end{enumerate}

    \end{enumerate}

  \item Given that this is the step response, and that it is multiplied by the step function, we know that:

    $$X(s)=\frac{1}{s}$$

    We take the transform of $y(t)$ to get:

    $$Y(s)=\frac{1}{s}-\frac{1}{s+2}-\frac{2}{(s+2)^2}$$

    We know that:

    $$H(s)=\frac{Y(s)}{H(s)}$$

    Thus, we find the transfer function be:

    $$H(s)=1-\frac{s}{s+2}-\frac{2s}{(s+2)^2}$$
    $$H(s)=\frac{4}{(s+2)^2}$$

    Then we can find:

    $$Y_1(s)=\frac{1}{s}-\frac{2}{s+2}+\frac{1}{s+4}$$

    Knowing that this must be equivalent to the transfer function, we see:

    $$\frac{Y_1(s)}{H(s)}=X_1(s)$$

    This gives us:

    $$X_1(s)=\frac{(s+2)^2}{4s}-.5(s+2)+\frac{(s+2)^2}{4(s+4)}$$
    $$X_1(s)=\frac{(s+2)^2}{4s}-.5(s+2)+\frac{(s+2)^2}{4s+16}$$

    We can simplify to get:

    $$X_1(s)=\frac{2s+4}{s^2+4s}$$
    $$X_1(s)=\frac{2}{s+4}+\frac{4}{s(s+4)}$$

    We use partial fraction decomposition for the second term to get:

    $$X_1(s)=\frac{2}{s+4}+\frac{A}{s+4}+\frac{B}{s}$$

    We find $A=-1$ and $B=1$ to get:

    $$X_1(s)=\frac{1}{s+4}+\frac{1}{s}$$

    Taking the inverse, we find:

    $$\boxed{x_1(t)=[e^{-4t}+1]u(t)}$$

  \item

    We may express $x(t)$ as:

    $$x(t)=e^{t}u(-t)+e^{-t}u(t)$$

    This gives us:

    $$X(s)=-\frac{1}{s-1}+\frac{1}{s+1}$$

    We combine the two terms to get:

    $$X(s)=\frac{-2}{s^2-1}$$

    Multiplying by the system function, we get:

    $$Y(s)=\left[ \frac{s+1}{s^2+2s+9} \right]\left[ -\frac{2}{s^2-1} \right]$$

    We continue to simplify:

    $$Y(s)=\left[ \frac{1}{s^2+2s+9} \right]\left[ -\frac{2}{s-1} \right]$$
    $$Y(s)=\frac{-2}{(s^2+2s+9)(s-1)}$$

    We then use partial fraction decomposition to write:

    $$Y(s)=\frac{A}{s-1}+\frac{Bs+C}{s^2+2s+9}$$

    Thus, we get:

    $$A(s^2+2s+9)+(Bs+C)(s-1)=-2$$
    $$As^2+2As+9A+Bs^2-Bs+Cs-C=-2$$

    From this, we can set up the following system:

    $$A+B=0$$
    $$2A-B-C=0$$
    $$9A-C=-2$$

    Solving the system, we see: $A=-\frac{1}{6}$, $B=\frac{1}{6}$, and $C=\frac{1}{2}$, which gives us:

    $$Y(s)=\frac{-1/6}{s-1}+\frac{(1/6)s+(1/2)}{s^2+2s+9}$$

    We break this up further to see:

    $$Y(s)=\frac{-1/6}{s-1}+\frac{(1/6)s+(1/6)}{(s+1)^2+8}+\frac{(1/3)}{(s+1)^2+8}$$
    $$Y(s)=\frac{-1/6}{s-1}+\frac{(1/6)s+(1/6)}{(s+1)^2+8}+\frac{1}{\sqrt{8}}\frac{3\sqrt{8}}{(s+1)^2+8}$$

    We then use the Laplace tables, and the fact that the system is causal, to get:

    $$\boxed{y(t)=-\frac{1}{6}e^{t}u(t)+\frac{1}{6}e^{-t}\cos(\sqrt{8}t)u(t)+\frac{1}{3\sqrt{8}}e^{-t}\sin(\sqrt{8}t)u(t)}$$

  \item

    \begin{enumerate}

      \item We may observe that the left side of the diagram indicates poles, and the right side indicates zeros, while the $s^{-1}$ blocks are delays. We know that the transfer function may be written as:

        $$H(s)=\dfrac{\displaystyle \sum_{n=0}^Nb_ns^{-n}}{\displaystyle 1+\sum_{n=1}^{N}a_ns^{-n}}$$

        We may see that $N=2$, which gives us:

        $$H(s)=\dfrac{\displaystyle \sum_{n=0}^2b_ns^{-n}}{\displaystyle 1+\sum_{n=1}^{2}-a_ns^{-n}}$$

        First, we work to get the numerator:

        $$H(s)=\frac{1-s^{-1}-3s^{-2}}{1+\sum_{n=1}^{2}a_ns^{-n}}$$

        And then the denominator:

        $$H(s)=\frac{1-s^{-1}-3s^{-2}}{1+2s^{-1}+4s^{-2}}$$

        Multiplying both the numerator and denominator by $s^2$, we get:

        $$H(s)=\frac{s^2-s-3}{s^2+2s+4}$$

        We know that the transfer function is equivalent to:

        $$H(s)=\frac{Y(s)}{X(s)}$$

        This allows us to obtain the following:

        $$s^2X(s)-sX(s)-3X(s)=s^2Y(s)+2sY(s)+4Y(s)$$

        Taking the invers transform, we see:

        $$\boxed{\frac{d^2y(t)}{dt^2}+2\frac{dy(t)}{dt}+4y(t)=\frac{d^2x(t)}{dt^2}-\frac{dx(t)}{dt}-3x(t)}$$

      \item We know the system is stable if all poles are to the left of the $s$-plane. This gives us:

        $$s^2+2s+4=0$$

        Using the quadratic equation, we get:

        $$s=\frac{-2\pm\sqrt{4-4(1)(4)}}{2}$$
        $$s=-1\pm 3j$$

        Given the $-1$ real part, all poles are to the left of the $s$-plane, and, therefore, the \underline{system is stable}.

    \end{enumerate}

  \item

    \begin{enumerate}

      \item From the information,  we know $Y(s)=(2s^2+3s-4)Y_1(s)$, which allows us to write:

        $$\boxed{y(t)=2\frac{d^2y_1(t)}{dt^2}+3\frac{dy_1(t)}{dt}-4y_1(t)}$$

      \item From the figure, we may observe the following relationship:

        $$s^{-1}f(t)=y_1(t)$$

        This allows us to obtain:

        $$\boxed{f(t)=\frac{dy_1(t)}{dt}}$$

      \item Similar to part (b), we may observe the flow of the diagram to see:

        $$s^{-2}e(t)=y_1(t)$$
        $$e(t)=s^2y_1(t)$$

        This allows us to get:

        $$\boxed{e(t)=\frac{d^2y_1(t)}{dt^2}}$$

      \item Given parts (a), (b), and (c), we may write the original signal as:

        $$\boxed{y(t)=2e(t)+3f(t)-4y_1(t)}$$

      \item 

        We may combine the diagram and result from (d) to form the following figure:

        \begin{figure}[H]
          \centering
          \include{Figures/HW6-8e}
          \caption{Full System $(S)$ Diagram}
          \label{fig:2}
        \end{figure}

      \item From the provided form, we may write:

        $$H_1(s)=\frac{Y_1(s)}{X(s)}\quad\text{ and }\quad H_2(s)=\frac{Y(s)}{Y_1(s)}$$

        This gives us:

        $$(s+3)Y_1(s)=(2s-4)X(s)\Rightarrow (s+2)Y_1(s)=(s+1)Y(s)$$
        $$\frac{dy_1(t)}{dt}+3y_1(t)=2\frac{dx(t)}{dt}-4x(t)\Rightarrow \frac{dy_1(t)}{dt}+2y_1(t)=\frac{dy(t)}{dt}+y(t)$$

        From $H_2(s)$, we may obtain:

        \begin{figure}[H]
          \centering
          \include{Figures/HW6-8f}
          \caption{Representation of $H_2(s)$}
          \label{fig:3}
        \end{figure}

        We then combine this with $H_1(s)$ to get a full system flow:

        \begin{figure}[H]
          \centering
          \include{Figures/HW6-8f2}
          \caption{Representation of Full System, $H(s)$}
          \label{fig:4}
        \end{figure}

      \item Based on the given system, we may obtain:

        \begin{figure}[H]
          \centering
          \include{Figures/HW6-8g}
          \caption{Representation of Full System (Part g), $H(s)$}
          \label{fig:5}
        \end{figure}

    \end{enumerate}

  \item

    \begin{enumerate}

      \item We may begin by converting all of the components to the frequency domain:

        $$z_C=\frac{1}{sC}\quad\text{ and }\quad z_L=sL$$

        This gives us:

        $$R=1[\si{\ohm}],\, z_C=\frac{2}{s}[\si{\ohm}],\, z_l=.4s[\si{\ohm}]$$

        Given that the components are in parallel, we can find the equivalent impedance:

        $$z_{eq1}=\frac{z_Cz_L}{z_C+z_L}$$
        $$z_{eq1}=\frac{.8}{(2/s)+.4s}$$
        $$z_{eq1}=\frac{.8s}{2+.4s^2}$$

        And then:

        $$z_{eq}=\frac{Rz_{eq1}}{R+z_{eq1}}$$
        $$z_{eq}=\frac{z_{eq1}}{1+z_{eq1}}$$
        $$z_{eq}=\frac{.8s}{2+.8s+.4s^2}$$

        The voltage through each branch may be found by taking:

        $$v(t)=z_{eq}i_g(t)$$
        $$v(t)=\frac{.8si_g(t)}{2+.8s+.4s^2}$$

        We then divide by the impedance of the capacitor to find the current:

        $$i_o(t)=\frac{.4s^2i_g(t)}{2+.8s+.4s^2}$$

        We then find the transfer function:

        $$H(s)=\frac{i_o(s)}{i_g(t)}$$
        $$H(s)=\frac{.4s^2}{2+.8s+.4s^2}$$

        To simplify, we multiply both the numerator and denominator by 5:

        $$H(s)=\frac{2s^2}{10+4s+2s^2}$$
        $$\boxed{H(s)=\frac{s^2}{5+2s+s^2}}$$

      \item 

        Given that we know:

        $$H(s)=\frac{Y(s)}{X(s)}$$

        We may obtain:

        $$s^2X(s)=[5+2s+s^2]Y(s)$$

        This gives us:

        $$\boxed{\frac{d^2i_g(t)}{dt^2}=5i_o(t)+2\frac{di_o(t)}{dt}+\frac{d^2i_o(t)}{dt^2}}$$

      \item 

        We may obtain $I_o(s)$ using the transfer function:

        $$I_o(s)=\left[ \frac{s^2}{s^2+2s+5} \right]I_g(s)$$

        We take the Laplace transform for the current input to get:

        $$I_g(s)=\frac{10s}{s^2+1}$$

        Multiplying, we get:

        $$\boxed{I_o(s)=\frac{10s^3}{(s^2+1)(s^2+2s+5)}}$$

      \item 

        We may begin by using partial fraction decomposition, such that:

        $$I_o(s)=\frac{As+B}{s^2+1}+\frac{Cs+D}{s^2+2s+5}$$

        Multiplying together, we find:

        $$Cs^3+Cs+Ds^2+D+As^3+2As^2+5As+Bs^2+2Bs+5B=10s^3$$

        This allows us to generate the following system:

        $$C+A=10$$
        $$D+2A+B=0$$
        $$C+5A+2B=0$$
        $$D+5B=0$$

        We solve the system and find: $A=-2, B=-1, C=12$, and $D=5$, which gives us:

        $$I_o(s)=\frac{-2s-1}{s^2+1}+\frac{12s+5}{s^2+2s+5}$$

        Continuing to simplify to take the inverse, we get:

        $$I_o(s)=-\frac{2s+1}{s^2+1}+\frac{12s+5}{(s+1)^2+2^2}$$
        $$I_o(s)=-\frac{2s}{s^2+1}-\frac{1}{s^2+1}+\frac{12(s+1)}{(s+1)^2+2^2}-\frac{7}{(s+1)^2+2^2}$$

        Per our tables, this gives us:

        $$\boxed{i_o(t)=[\underbrace{-2\cos(t)-\sin(t)}_{\text{steady-state}}+\overbrace{12e^{-t}\cos(2t)-7e^{-t}\sin(2t)}^{\text{transient}}]u(t)}$$

        The transient terms fade with time and are expressed as those with decaying exponentials, while the steady state response is purely sinusoidal.

    \end{enumerate}

\end{enumerate}

\end{document}

