%%%%%%%%%%%%%%%%%%%%%%%%%%%%%%%%%%%%%%%%%%%%%%%%%%%%%%%%%%%%%%%%%%%%%%%%%%%%%%%%%%%%%%%%%%%%%%%%%%%%%%%%%%%%%%%%%%%%%%%%%%%%%%%%%%%%%%%%%%%%%%%%%%%%%%%%%%%%%%%%%%%
% Written By Michael Brodskiy
% Class: Fundamentals of Linear Systems
% Professor: I. Salama
%%%%%%%%%%%%%%%%%%%%%%%%%%%%%%%%%%%%%%%%%%%%%%%%%%%%%%%%%%%%%%%%%%%%%%%%%%%%%%%%%%%%%%%%%%%%%%%%%%%%%%%%%%%%%%%%%%%%%%%%%%%%%%%%%%%%%%%%%%%%%%%%%%%%%%%%%%%%%%%%%%%

\include{Includes.tex}

\title{Homework 1}
\date{\today}
\author{Michael Brodskiy\\ \small Professor: I. Salama}

\begin{document}

\maketitle

\begin{enumerate}

  \item Express each of the following complex numbers in polar form and plot them

    \begin{enumerate}

      \item $8$

        $$r=\sqrt{8^2+0^2}=8$$
        $$\theta=0$$
        $$z(r,\theta)=r(\cos(\theta)+j\sin(\theta))$$
        $$z(8,0)=8(\cos(0)+j\sin(0))$$
        $$\therefore \text{ In polar: } \boxed{z=8}$$

        \begin{figure}[H]
          \centering
          \include{Figures/Fig1a}
          \caption{$z=8$ Plotted on the Imaginary Plane}
          \label{fig:1}
        \end{figure}

      \item $-5$

        $$r=\sqrt{(-5)^2+0^2}=5$$
        $$\theta=\pi$$
        $$z(r,\theta)=r(\cos(\theta)+j\sin(\theta))$$
        $$z(5,\pi)=5(\cos(\pi)+j\sin(\pi))$$
        $$\therefore \text{ In polar: } \boxed{z=-5=5e^{\pi j}}$$

        \begin{figure}[H]
          \centering
          \include{Figures/Fig1b}
          \caption{$z=-5$ Plotted on the Imaginary Plane}
          \label{fig:2}
        \end{figure}

      \item $2j$

        $$r=\sqrt{0^2+(2)^2}=2$$
        $$\theta=\frac{\pi}{2}$$
        $$z(r,\theta)=r(\cos(\theta)+j\sin(\theta))$$
        $$z(2,.5\pi)=2j$$
        $$\therefore \text{ In polar: } \boxed{z=2j=2e^{.5\pi j}}$$

        \begin{figure}[H]
          \centering
          \include{Figures/Fig1c}
          \caption{$z=2j$ Plotted on the Imaginary Plane}
          \label{fig:3}
        \end{figure}

      \item $\frac{1}{4}(1-j)^5$

        $$.25(1-j)^2(1-j)^3$$
        $$.25(-2j)(1-j)(1-j)^2$$
        $$.25(-2-2j)(-2j)$$
        $$z=j-1$$
        $$r=\sqrt{1^2+(-1)^2}=\sqrt{2}$$
        $$\theta=\frac{3\pi}{4}$$
        $$z(r,\theta)=r(\cos(\theta)+j\sin(\theta))$$
        $$z(\sqrt{2},.75\pi)=j-1$$
        $$\therefore \text{ In polar: } \boxed{z=j-1=\sqrt{2}e^{.75\pi j}}$$

        \begin{figure}[H]
          \centering
          \include{Figures/Fig1d}
          \caption{$z=\frac{1}{4}(1-j)^5$ Plotted on the Imaginary Axis}
          \label{fig:4}
        \end{figure}

      \item $\frac{(1+j)}{j}e^{\frac{j\pi}{3}}$

        $$\frac{(1+j)}{j}\cdot\frac{-j}{-j}=1-j$$
        $$\tan\left( \frac{\pi}{3} \right)=\frac{b}{a}$$
        $$\frac{b}{a}=\sqrt{3}$$
        $$b=a\sqrt{3}$$
        $$\sqrt{(a\sqrt{3})^2+a^2}=1$$
        $$4a^2=\pm1$$
        $$a=\frac{1}{2}$$
        $$b=\frac{\sqrt{3}}{2}$$
        $$\frac{1}{2}(1-j)(1+\sqrt{3}j)\to\frac{1}{2}((\sqrt{3}+1)+(\sqrt{3}-1)j)$$
        $$r=\frac{1}{2}\sqrt{(\sqrt{3}+1)^2+(\sqrt{3}-1)^2}=\sqrt{(4+2\sqrt{3})+(4-2\sqrt{3})}$$
        $$r=\sqrt{2}$$
        $$\theta=\tan^{-1}\left( \frac{\sqrt{3}-1}{\sqrt{3}+1} \right)=.26179$$
        $$z(r,\theta)=r(\cos(\theta)+j\sin(\theta))$$
        $$z(\sqrt{2},.26179)=\frac{1}{2}(\sqrt{3}+1)+(\sqrt{3}-1)j$$
        $$\therefore \text{ In polar: } \boxed{z=\frac{1}{2}(\sqrt{3}+1)+(\sqrt{3}-1)j=\sqrt{2}e^{.26179j}}$$

        \begin{figure}[H]
          \centering
          \include{Figures/Fig1e}
          \caption{$z=\frac{(1+j)}{j}e^{\frac{j\pi}{3}}$ Plotted on the Imaginary Axis}
          \label{fig:5}
        \end{figure}

      \item $(\sqrt{3}-j^5)(1+j)$

        $$j^5=j\to (\sqrt{3}-j)(1+j)=(\sqrt{3}+(\sqrt{3}-1)j+1)$$
        $$(\sqrt{3}+1)+(\sqrt{3}-1)j$$
        $$r=\sqrt{(\sqrt{3}+1)^2+(\sqrt{3}-1)^2}=\sqrt{(4+2\sqrt{3})+(4-2\sqrt{3})}$$
        $$r=\sqrt{8}=2\sqrt{2}$$
        $$\theta=\tan^{-1}\left( \frac{\sqrt{3}-1}{\sqrt{3}+1} \right)=.26179$$
        $$z(r,\theta)=r(\cos(\theta)+j\sin(\theta))$$
        $$z(2\sqrt{2},.26179)=(\sqrt{3}+1)+(\sqrt{3}-1)j$$
        $$\therefore \text{ In polar: } \boxed{z=(\sqrt{3}+1)+(\sqrt{3}-1)j=2\sqrt{2}e^{.26179j}}$$

        \begin{figure}[H]
          \centering
          \include{Figures/Fig1f}
          \caption{$z=(\sqrt{3}-j^5)(1+j)$ Plotted on the Imaginary Axis}
          \label{fig:6}
        \end{figure}

      \item $\frac{2(\sqrt{3}-j)}{1+j\sqrt{3}}$

        $$\frac{2\sqrt{3}-2j}{1+j\sqrt{3}}\cdot\frac{1-j\sqrt{3}}{1-j\sqrt{3}}=-2j$$
        $$r=\sqrt{0^2+(-2)^2}=2$$
        $$\theta=\frac{3\pi}{2}$$
        $$z(r,\theta)=r(\cos(\theta)+j\sin(\theta))$$
        $$z(2,1.5\pi)=-2j$$
        $$\therefore \text{ In polar: } \boxed{z=-2j=2e^{1.5\pi j}}$$

        \begin{figure}[H]
          \centering
          \include{Figures/Fig1g}
          \caption{$z=\frac{2(\sqrt{3}-j)}{1+j\sqrt{3}}$ Plotted on the Imaginary Axis}
          \label{fig:7}
        \end{figure}

    \end{enumerate}

  \item Determine the value of $E_{\infty}$ and $P_{\infty}$ for each of the following signals and indicate whether the signal is a power or energy signal or neither.

    \begin{enumerate}

      \item $x_1(t)=\left\{\begin{array}{l r} 5e^{j(4t+\pi/3)},\, & t\geq 2\\ 0,\, & \text{Otherwise}\end{array}$

          $$|x_1(t)|=\sqrt{\left( 5\cos\left( 4t+\frac{\pi}{3} \right) \right)^2+\left( 5\sin\left( 4t+\frac{\pi}{3} \right) \right)^2}$$
          $$|x_1(t)|=5\sqrt{2}$$

          $$E_{\infty}=\int_2^{\infty} 50\,dt$$
          $$E_{\infty}=\infty$$
          $$\therefore\text{ Energy is infinite}$$

          $$P_{\infty}=\lim_{T\to\infty}\frac{1}{T}\int_{-T/2}^{T/2}50\,dt$$
          $$P_{\infty}=50$$
          $$\therefore\text{ Power is finite}$$

          $$\boxed{\text{Therefore, this is a power signal}}$$

      \item $x_2(t)=\left\{\begin{array}{l r} 2+2\cos(t),\, & 0<t< 2\pi\\ 0,\, & \text{Otherwise}\end{array}$

          $$P_{\infty}=\lim_{T\to\infty}\frac{1}{2T}\int_{-T}^{T}(2+2\cos(t))^2\,dt$$
          $$P_{\infty}=6$$
          $$\therefore\text{ Power is finite}$$

          $$E_{\infty}=\lim_{T\to\infty}\int_{-T}^T(2+2\cos(t))^2\,dt$$
          $$E_{\infty}=\infty$$
          $$\therefore\text{ Energy is infinite}$$

          \begin{center}
            $$\boxed{\text{Since power is finite and energy is infinite, this is a power signal}}$$
          \end{center}

        \item $x_3[n]=\left\{\begin{array}{l r} (.5)^n,\, & n\geq0\\ 0,\, & \text{Otherwise}\end{array}$

            $$E_{\infty}=\lim_{N\to\infty}\sum_{n=0}^N \left( .25 \right)^n$$
            \begin{center}
              A geometric series must be finite:
            \end{center}
            $$E_{\infty}\approx \left( \frac{1}{1-.25} \right)\approx \frac{4}{3}$$

            $$P_{\infty}=\lim_{N\to\infty}\frac{4/3}{2N+1}\approx 0$$

            \begin{center}
              $\boxed{\text{As such, because energy is finite and average power is 0, this is an energy signal}}$
            \end{center}

    \end{enumerate}

  \item For the discrete time signal shown in Figure P1.3, sketch, and carefully label each of the following.

    \begin{enumerate}

      \item $x[n-4]$

        \begin{figure}[H]
          \centering
          \include{Figures/Fig3a}
          \label{fig:8}
        \end{figure}

      \item $x[2n+2]$

        \begin{figure}[H]
          \centering
          \include{Figures/Fig3b}
          \label{fig:9}
        \end{figure}

    \end{enumerate}

  \item For the continuous time signal shown in Figure P1.4, sketch, and carefully label each of the following.

    \begin{enumerate}

      \item $x(t+3)$

        \begin{figure}[H]
          \centering
          \include{Figures/Fig4a}
          \caption{Figure Showing Transformation $x(t)\to x(t+3)$}
          \label{fig:10}
        \end{figure}

      \item $x\left( 3-\frac{2}{3}t \right)$

        \begin{figure}[H]
          \centering
          \include{Figures/Fig4b}
          \caption{Figure Showing Transformation $x(t)\to x\left( 3-\frac{2}{3}t \right)$}
          \label{fig:11}
        \end{figure}

    \end{enumerate}

  \item Determine and sketch the even and odd parts of the signals depicted in Figure P1.5. Label your sketches carefully.

    \begin{enumerate}

      \item The original plot is as follows:

        \begin{figure}[H]
          \centering
          \include{Figures/Fig5a1}
          \caption{Original Plot}
          \label{fig:12}
        \end{figure}

        First, we begin by plotting $x(-t)$:

        \begin{figure}[H]
          \centering
          \include{Figures/Fig5a2}
          \caption{$x(t)\to x(-t)$}
          \label{fig:13}
        \end{figure}

        From here, we find the average of the two to find the even part:

        $$\frac{x(t)+x(-t)}{2}\to\frac{-2t+2t}{2}=0$$

        Thus, we see there is no even part (the plot would show $x(t)=0$ for $0<t<1$).

        From here, we subtract $x(-t)$ from $x(t)$ and then divide by two:

        $$\frac{x(t)-x(-t)}{2}\to\frac{2t-(-2t)}{2}=2t$$

        We can plot this; however, as a result of being purely an even function, the plot would be the same as the original:

        \begin{figure}[H]
          \centering
          \include{Figures/Fig5a3}
          \caption{$x(t)$ Even (Original Plot)}
          \label{fig:14}
        \end{figure}

      \item The original plot is as follows:

        \begin{figure}[H]
          \centering
          \include{Figures/Fig5b1}
          \caption{Original Plot}
          \label{fig:15}
        \end{figure}

        First, we begin by plotting $x(-t)$:

        \begin{figure}[H]
          \centering
          \include{Figures/Fig5b2}
          \caption{$x(t)\to x(-t)$}
          \label{fig:16}
        \end{figure}

        From here, we find the average of the two to find the even part:

        $$\frac{x(t)+x(-t)}{2}\to\frac{-2t-t}{2}=-\frac{3t}{2}\text{ for }t<0$$
        $$\frac{x(t)+x(-t)}{2}\to\frac{2t+t}{2}=\frac{3t}{2}\text{ for }t>0$$

        Then, we plot this:

        \begin{figure}[H]
          \centering
          \include{Figures/Fig5b3}
          \caption{Even $x(t)$}
          \label{fig:17}
        \end{figure}

        From here, we subtract $x(-t)$ from $x(t)$ and then divide by two:

        $$\frac{x(t)-x(-t)}{2}\to\frac{-2t+t}{2}=-\frac{t}{2}\text{ for }t<0$$
        $$\frac{x(t)-x(-t)}{2}\to\frac{t-2t}{2}=-\frac{t}{2}\text{ for }t>0$$

        Then, we plot this:

        \begin{figure}[H]
          \centering
          \include{Figures/Fig5b4}
          \caption{Odd $x(t)$}
          \label{fig:18}
        \end{figure}

        Hence, we have the even and odd figures here.

    \end{enumerate}

  \item Determine and sketch the even and odd parts of the signal depicted in Figure P1.6. Label your sketches carefully.

    For this problem, we find even using:

    $$\frac{x[n]+x[-n]}{2}$$

    and the odd part with:

    $$\frac{x[n]-x[-n]}{2}$$

    The original signal is as follows:

        \begin{figure}[H]
          \centering
          \include{Figures/Fig6}
          \caption{Original Plot}
          \label{fig:19}
        \end{figure}

        Using the above formulas, we can draw the even:

        \begin{figure}[H]
          \centering
          \include{Figures/Fig6-1}
          \caption{Even $x[n]$}
          \label{fig:20}
        \end{figure}

        and then the odd:

        \begin{figure}[H]
          \centering
          \include{Figures/Fig6-2}
          \caption{Odd $x[-n]$}
          \label{fig:21}
        \end{figure}

  \item Express the real part of each of the following signals in the form $Ae^{-at}\cos(\omega t + \phi)$ where $A$, $a$, $\omega$ and $\phi$ are real numbers with $A > 0$ and $-\pi < \phi \leq \pi$.

    \begin{enumerate}

      \item $x_1(t)=4e^{-2t}\sin\left( 10t+\frac{3\pi}{4}\right)\cos\left( 10t+\frac{3\pi}{4} \right)$

        \begin{center}
          Per trig identities, we can rewrite this as:
        \end{center}
        $$2e^{-2t}\sin\left( 20t+\frac{3\pi}{2}\right) \right)$$
        \begin{center}
          Per another identity, we can convert $\sin\to\cos$:
        \end{center}
        $$2e^{-2t}\cos\left( \frac{\pi}{2}-20t-\frac{3\pi}{2}\right) \right)$$
        $$x_1(t)=2e^{-2t}\cos\left( -20t-\pi\right) \right)$$
        \begin{center}
          Since $\cos(x)=\cos(-x)$, we finally write:
        \end{center}
        $$\boxed{x_1(t)=2e^{-2t}\cos\left( 20t+\pi\right) \right)}$$

      \item $x_2(t)=j(1-j)e^{(-5+j\pi)t}$

        We can rewrite this in terms of exponentials:

        $$x_2(t)=e^{\frac{\pi}{2}j}\left( \sqrt{2}e^{-\frac{\pi}{4}j} \right)\left( e^{(-5+j\pi)t} \right)$$
        $$x_2(t)=\sqrt{2}e^{-5t}\left( e^{j\pi t+\frac{\pi}{2}j-\frac{\pi}{4}j} \right)$$
        $$x_2(t)=\sqrt{2}e^{-5t}\left( e^{j(\pi t+\frac{\pi}{4})} \right)$$
        $$\boxed{x_2(t)=\sqrt{2}e^{-5t}\cos\left(\pi t+\frac{\pi}{4}\right)}$$

    \end{enumerate}

  \item Determine whether each of the following continuous time signals is periodic. If the signal is periodic, determine its fundamental period.

    \begin{enumerate}

      \item $x(t)=5\cos\left( 400\pi t+\frac{\pi}{4} \right)$

        The function is periodic, with angular frequency $\omega=400\pi\left[ \dfrac{\text{rad}}{\si{\second}} \right]$

        This gives us the fundamental period:

        $$\boxed{T=\frac{2\pi}{400\pi}=.005[\si{\second}]}$$

      \item $x(t)=20e^{j(\pi t-2)}$

        The function is periodic, with angular frequency $\omega=\pi\left[ \dfrac{\text{rad}}{\si{\second}} \right]$

        This gives us the fundamental period:

        $$\boxed{T=\frac{2\pi}{\pi}=2[\si{\second}]}$$

      \item $x(t)=2\left[ \sin\left( 50\pi t - \frac{\pi}{3} \right) \right]^2$

        The function is periodic, with angular frequency $\omega=50\pi\left[ \dfrac{\text{rad}}{\si{\second}} \right]$

        This gives us the fundamental period:

        $$\boxed{T=\frac{2\pi}{50\pi}=.04[\si{\second}]}$$

      \item $x(t)=\left\{\begin{array}{l r} 2\sin(5\pi t),\, & t\geq 0\\ -2\sin(-5\pi t),\, &t<0\end{array}$

        Per trigonometric identities, we know that:

        $$\sin(t)=-\sin(-t)$$

        Thus, the function presented is simply:

        $$x(t)=2\sin(5\pi t)$$

        This function is periodic, with angular frequency $\omega=5\pi\left[ \dfrac{\text{rad}}{\si{\second}} \right]$

        This gives us the fundamental period:

        $$\boxed{T=\frac{2\pi}{5\pi}=.4[\si{\second}]}$$

    \end{enumerate}

  \item Determine whether each of the following discrete time signals is periodic. If the signal is periodic, determine its fundamental period.

    \begin{enumerate}

      \item $x[n]=2\cos\left( \frac{7}{11}n+\frac{\pi}{2} \right)$

        To be periodic, $(2\pi/\Omega_o)m$ must be rational. We see:

        $$\Omega_o=\frac{7}{11}\to\frac{22\pi m}{7}$$

        As a result of the $\pi$, this is never rational and therefore not periodic.

      \item $x[n]=\cos(\pi n)+4\sin\left( \frac{\pi}{4}n^2 \right)$

        To be periodic, both sinusoids must have $2\pi/\Omega_o$ be rational. We see:

        $$\Omega_1=\pi\to\frac{2\pi}{\pi}=2\text{ and }\Omega_2=\pi/4\to\frac{2\pi}{\pi/4}=8$$

        Thus, the function is periodic. The period is the smallest number such that the two periods are a common divisor of the integer. Since 8 is divisible by 2, \underline{the fundamental period is 8}.

      \item $x[n]=3\sin\left( \frac{\pi}{3}n \right)+\cos\left( \frac{\pi}{4}n \right)-3\cos\left( \frac{\pi}{6}n+\frac{\pi}{3} \right)$ 

        Once again, each of the sinusoids must be periodic:

        $$\Omega_1=\pi/3\to\frac{2\pi}{\pi/3}=6\text{ and }\Omega_2=\pi/4\to\frac{2\pi}{\pi/4}=8\text{ and }\Omega_3=\pi/6\to\frac{2\pi}{\pi/6}=12$$

        Thus, we see these functions are all periodic. The smallest integer which is divisible by all of these values is 24, and, thus, \underline{the fundamental period is 24}.

    \end{enumerate}

\end{enumerate}

\end{document}

