%%%%%%%%%%%%%%%%%%%%%%%%%%%%%%%%%%%%%%%%%%%%%%%%%%%%%%%%%%%%%%%%%%%%%%%%%%%%%%%%%%%%%%%%%%%%%%%%%%%%%%%%%%%%%%%%%%%%%%%%%%%%%%%%%%%%%%%%%%%%%%%%%%%%%%%%%%%%%%%%%%%
% Written By Michael Brodskiy
% Class: Fundamentals of Linear Systems
% Professor: I. Salama
%%%%%%%%%%%%%%%%%%%%%%%%%%%%%%%%%%%%%%%%%%%%%%%%%%%%%%%%%%%%%%%%%%%%%%%%%%%%%%%%%%%%%%%%%%%%%%%%%%%%%%%%%%%%%%%%%%%%%%%%%%%%%%%%%%%%%%%%%%%%%%%%%%%%%%%%%%%%%%%%%%%

\include{Includes.tex}

\title{Homework 3}
\date{\today}
\author{Michael Brodskiy\\ \small Professor: I. Salama}

\begin{document}

\maketitle

\begin{enumerate}

  \item Classifying systems as memory-less, time-invariant, linear, causal, and/or stable:

    \begin{enumerate}

      \item $y(t)=5e^{4t}x(t-1)$

        \begin{itemize}

          \item Memory: \textbf{not} memory-less; the $x(t-1)$ term means the system relies on values other than the present value; therefore, it is not memory-less

          \item Time-Invariant: \textbf{not} time-invariant; we may see that, $y(t-t_o)$ changes the $t$ value in the exponential and $x(t)$ statement, while $x(t-t_o)$ changes only the $x(t)$ statement; thus, it is not time-invariant, since $x(t-t_o)\neq y(t-t_o)$

          \item Linear: the system \textbf{is} linear (see below) because $ax_1(t)+bx_2(t)= ay_1(t)+by_2(t)$

            $$ax_1(t)+bx_2(t)\to a5e^{4t}x_1(t-1)+b5e^{4t}x_2(t-1)$$
            $$ay_1(t)+by_2(t)\to a5e^{4t}x_1(t-1)+b5e^{4t}x_2(t-1)$$

          \item Causal: the system \textbf{is} causal , because it only depends on past or present values (ex. $t=0\to y(t)=5e^{4(0)}x(-1)$)

          \item Stable: Given that the system depends on an exponential $e^{4t}$, its maximum value is unbounded and, therefore, it is \textbf{unstable}

        \end{itemize}

      \item $y(t)=\displaystyle \int_{-\infty}^{\frac{t}{2}} x(\tau)\,d\tau$

        \begin{itemize}

          \item Memory: \textbf{not} memory-less; the system depends on a shift of the $t$ parameter ($t/2$), and, therefore, does not always depend on the current value of time

          \item Time-Invariant: \textbf{not} time-invariant; $y(t-t_o)\neq x(t-t_o)$ (see below)

            $$x(t-t_o)\to \int_{-\infty}^{\frac{t}{2}} x(\tau-t_o)\,d\tau$$
            $$y(t-t_o)\to \int_{-\infty}^{\frac{(t-t_o)}{2}} x(\tau-t_o)\,d\tau$$
            $$\therefore x(t-t_o)\neq y(t-t_o)$$

          \item Linear: the system \textbf{is} linear; it follows both the superposition and homogeneity principles (see below)

            $$ay_1(t)+by_2(t)\to a\int_{-\infty}^{\frac{t}{2}} x_1(\tau)\,d\tau+b\int_{-\infty}^{\frac{t}{2}} x_2(\tau)\,d\tau$$
            $$ax_1(t)+bx_2(t)\to a\int_{-\infty}^{\frac{t}{2}} x_1(\tau)\,d\tau+b\int_{-\infty}^{\frac{t}{2}} x_2(\tau)\,d\tau$$
            $$\therefore ax_1(t)+bx_2(t)=ay_1(t)+by_2(t)$$

          \item Causal: the system \textbf{is not} causal; integration depends on future values when $t<0$

          \item Stable: the system \textbf{is not} stable (see below)

            $$y(t)=\int_{-\infty}^{\frac{t}{2}} x(\tau)\,d\tau$$
            $$h(t)=\int_{-\infty}^{\frac{t}{2}} \delta(\tau)\,d\tau=\left\{\begin{array}{ll}0,& t<0\\1,& t>0\end{array}$$
            $$h(t)\to u(t)$$
            $$\int_{-\infty}^{\infty} h(t)\,dt=\infty$$

        \end{itemize}

      \item $y(t)=4+5\dfrac{d^2}{dt^2}x(t)$

        \begin{itemize}

          \item Memory: the system is \textbf{not} memory-less; the use of a differential implies that the system depends on past values

          \item Time-Invariant: the system \textbf{is} time-invariant (see below)

            $$x(t-t_o)\to 4+5\dfrac{d^2}{dt^2}x(t-t_o)$$
            $$y(t-t_o)\to 4+5\dfrac{d^2}{dt^2}x(t-t_o)$$
            $$\therefore x(t-t_o)=y(t-t_o)$$

          \item Linear: the system is \textbf{not} linear (see below)

            $$ax_1(t)+bx_2(t)=\left(4+5a\dfrac{d^2}{dt^2}x_1(t)\right)+\left(4+5b\dfrac{d^2}{dt^2}x_2(t)\right)$$
            $$ay_1(t)+by_2(t)=a\left(4+5\dfrac{d^2}{dt^2}x_1(t)\right)+b\left(4+5\dfrac{d^2}{dt^2}x_2(t)\right)$$
            $$\therefore ax_1(t)+bx_2(t)\neq ay_1(t)+by_2(t)$$

          \item Causal: the system \textbf{is} causal because it only depends on past or present values

          \item Stable: the system is \textbf{unstable} because it is unbounded

        \end{itemize}

      \item $y(t)=\left\{\begin{array}{ll} 0, & t<0\\ x(t-2)+2x(t), & t\geq0\end{array}$

        \begin{itemize}

          \item Memory: the system is \textbf{not} memory-less, since the $x(t-2)$ term depends on a past value

          \item Time-Invariant: the system is \textbf{not} time-invariant (see below)

            $$x(t-t_o)\to\left\{\begin{array}{ll} 0, & t<0\\ x(t-2-t_o)+2x(t-t_o), & t\geq0\end{array}$$
            $$y(t-t_o)\to\left\{\begin{array}{ll} 0, & t<2\\ x(t-2-t_o)+2x(t-t_o), & t\geq2\end{array}$$
            $$\therefore x(t-t_o)\neq y(t-t_o)$$

          \item Linear: the system \textbf{is} linear (see below)

            $$ax_1(t)+bx_2(t)\to\left\{\begin{array}{ll} 0, & t<0\\ ax_1(t-2)+2ax_1(t)+bx_2(t-2)+2bx_2(t), & t\geq0\end{array}$$
            $$ay_1(t)+by_2(t)\to\left\{\begin{array}{ll} 0, & t<0\\ ax_1(t-2)+2ax_1(t)+bx_2(t-2)+2bx_2(t), & t\geq0\end{array}$$
              $$\therefore ax_1(t)+bx_2(t)=ay_1(t)+by_2(t)$$

            \item Causal: the system \textbf{is} causal because it only depends on past or present values

            \item Stable: the system \textbf{is} stable, because it does not tend to diverge

        \end{itemize}

        Problem 1 can be tabulated as follows:

        \begin{center}
          \begin{tabular}[H]{|c|c|c|c|c|}
            \hline
            System & a & b & c & d\\
            \hline
            Memory-Less & no & no & no & no\\
            \hline
            Time-Invariant & no & no & yes & no\\
            \hline
            Linear & yes & yes & no & yes\\
            \hline
            Causal & yes & no & yes & yes\\
            \hline
            Stable & no & no & no & yes\\
            \hline
          \end{tabular}
        \end{center}

    \end{enumerate}

  \item Classifying systems as memory-less, time-invariant, linear, causal, and/or stable:

    \begin{enumerate}

      \item $y[n]=x[n+1]-2x[n-4]$

        \begin{itemize}

          \item Memory: system is \textbf{not} memory-less, as it depends on past and future values

          \item Time-Invariant: system \textbf{is} time-invariant (see below)

            $$x[n-n_o]=x[n+1-n_o]-2x[n-4-n_o]$$
            $$y[n-n_o]=x[n+1-n_o]-2x[n-4-n_o]$$
            $$\therefore x[n-n_o]=y[n-n_o]$$

          \item Linear: system \textbf{is} linear (see below)

            $$ax_1[n]+bx_2[n]=a(x_1[n+1]-2x_1[n-4])+b(x_2[n+1]-2x_2[n-4])$$
            $$ay_1[n]+by_2[n]=a(x_1[n+1]-2x_1[n-4])+b(x_2[n+1]-2x_2[n-4])$$
            $$\therefore ay_1[n]+by_2[n]=ax_1[n]+bx_2[n]$$

          \item Causal: system is \textbf{not} causal, as it depends on past and present values

          \item Stable: system \textbf{is} stable because $y[n]$ is finite

        \end{itemize}

      \item $y[n]=\text{Even}\left\{ x[n-1] \right\}$

        To simplify analysis, we can express the even function as:

        $$\frac{x[n]+x^*[-n]}{2}\to\frac{x[n-1]+x^*[-n+1]}{2}$$

        \begin{itemize}

          \item Memory: system is \textbf{not} memory-less, as it depends on future values

          \item Time-Invariant: system \textbf{is} time-invariant (see below)

            $$x[n-n_o]=\text{Even}\left\{ x[n-1-n_o] \right\}$$
            $$y[n-n_o]=\text{Even}\left\{ x[n-1-n_o] \right\}$$
            $$\therefore x[n-n_o]=y[n-n_o]$$

          \item Linear: system is \textbf{not} linear (see below); note that this is because $a$ or $b$ may be complex. Given this, for a purely real signal, the system can be classified as linear; however, due to the need to use the 'conjugate' for the even function, in the case of a complex signal, this is non-linear

            $$ax_1[n]+bx_2[n]=\frac{ax_1[n-1]+a^*x_1^*[-n+1]}{2}+\frac{bx_2[n-1]+b^*x_2^*[-n+1]}{2}$$
            $$ay_1[n]+by_2[n]=\frac{ax_1[n-1]+ax_1^*[-n+1]}{2}+\frac{bx_2[n-1]+bx_2^*[-n+1]}{2}$$
            $$\therefore ay_1[n]+by_2[n]\neq ax_1[n]+bx_2[n]$$

          \item Causal: system is \textbf{not} causal, as it depends on a future value

          \item Stable: system \textbf{is} stable because $y[n]$ is finite

        \end{itemize}

      \item $y[n]=5x[3n+1]$

        \begin{itemize}

          \item Memory: system is \textbf{not} memory-less, as it depends on non-present values

          \item Time-Invariant: system is \textbf{not} time-invariant (see below)

            $$x[n-n_o]=5x[3n-n_o+1]$$
            $$y[n-n_o]=5x[3n-3n_o+1]$$
            $$\therefore x[n-n_o]\neq y[n-n_o]$$

          \item Linear: system \textbf{is} linear (see below)

            $$ax_1[n]+bx_2[n]=5ax_1[3n+1]+5bx_2[3n+1]$$
            $$ay_1[n]+by_2[n]=5ax_1[3n+1]+5bx_2[3n+1]$$
            $$\therefore ay_1[n]+by_2[n]=ax_1[n]+bx_2[n]$$

          \item Causal: system is \textbf{not} causal, as it depends on a future value

          \item Stable: system \textbf{is} stable because $y[n]$ is finite

        \end{itemize}

      \item $y[n]=\left\{ \begin{array}{ll} 0, & n=2\\ x[n], & \text{otherwise}\end{array}$

        \begin{itemize}

          \item Memory: system \textbf{is} memory-less; it does not depend on past or present values

          \item Time-Invariant: system is \textbf{not} time-invariant (see below)

            $$x[n-n_o]=\left\{ \begin{array}{ll} 0, & n=2\\ x[n-n_o], & \text{otherwise}\end{array}$$
            $$y[n-n_o]=\left\{ \begin{array}{ll} 0, & n=2+n_o\\ x[n-n_o], & \text{otherwise}\end{array}$$
            $$\therefore x[n-n_o]\neq y[n-n_o]$$

          \item Linear: system \textbf{is} linear (see below)

            $$ax_1[n]+bx_2[n]=\left\{ \begin{array}{ll} 0, & n=2\\ ax_1[n]+bx_2[n], & \text{otherwise}\end{array}$$
            $$ay_1[n]+by_2[n]=\left\{ \begin{array}{ll} 0, & n=2\\ ax_1[n]+bx_2[n], & \text{otherwise}\end{array}$$
            $$\therefore ay_1[n]+by_2[n]=ax_1[n]+bx_2[n]$$

          \item Causal: system \textbf{is} causal, as it depends on only past or present values

          \item Stable: system \textbf{is} stable because $y[n]$ is finite

        \end{itemize}

    \end{enumerate}

  \item

    \begin{enumerate}

      \item 

        We may begin by constructing the expression for the convolution sum:

        $$y[n]=\sum_{k=-\infty}^{\infty}x[k]h[n-k]$$

        This gets us:

        $$y[n]=\sum_{k=-\infty}^{\infty} \left( \frac{1}{4} \right)^{k-2}u[k-2]u[n-k+1]$$

        We may observe the following:

        $$x[n]\neq 0,\quad n\geq 2$$
        $$h[n]\neq 0,\quad n\geq -1$$

        Integrating this into the convolution sum, we may see that the expression is nonzero (unit functions both exist) for $k\geq 2$, and that $k\leq n+1$. Thus, we get:

        $$y[n]=\sum_{k=2}^{n+1} \left( \frac{1}{4} \right)^{k-2}$$

        Using the expansion for series, we obtain:

        $$y[n]=\frac{1-(.25)^{n-1}}{1-.25}$$
        $$\boxed{y[n]=\frac{4}{3}\left[ 1-\left( \frac{1}{4} \right)^{n-1} \right]\text{ for }n\geq 2}$$\\

        This can be sketched as:

        \begin{figure}[H]
          \centering
          \include{Figures/HW3-3a}
          \caption{Sketch of $y[n]$}
          \label{fig:1}
        \end{figure}

      \item 

        Per the time-shifting property, we know that:

        $$y[n]=x[n]*h[n]\to y_1[n]=y[n-3]=x[n-3]*h[n]$$

        Which gives us:

        $$\boxed{y_1[n]=\frac{4}{3}\left[ 1-\left( \frac{1}{4} \right)^{n-4} \right]\text{ for }n\geq 5}$$

      \item 

        Per the time-shifting property, we know that:

        $$y[n]=x[n]*h[n]\to y_2[n]=y[n-2]=x[n]*h[n-2]$$

        $$\boxed{y_2[n]=\frac{4}{3}\left[ 1-\left( \frac{1}{4} \right)^{n-3} \right]\text{ for }n\geq 4}$$

      \item 

        Per the time-shifting property, we know that:

        $$y[n]=x[n]*h[n]\to y_3[n]=y[n+1]=x[n-2]*h[n+3]$$

        $$\boxed{y_3[n]=\frac{4}{3}\left[ 1-\left( \frac{1}{4} \right)^{n} \right]\text{ for }n\geq 1}$$

    \end{enumerate}

  \item

    We may simplify analysis by using a tabulating method. Using this, we can see that:

    $$x=\left\{ 0, 1, 1, 1 \right\}$$
    $$h=\left\{ 0, 0, 0, 0, 0, 1, 1, 1, 1, 1, 1 \right\}$$

    This can be written as:

    \begin{center}
    \begin{tabular}[H]{c|cccc}
      & 0 & 1 & 1 & 1\\
      \hline
      0 & \iddots & \iddots & \iddots & \iddots \\
      0 & \iddots & \iddots & \iddots & \iddots \\
      0 & \iddots & \iddots & \iddots & \iddots \\
      0 & \iddots & \iddots & \iddots & \iddots \\
      0 & \iddots & \iddots & \iddots & \iddots \\
      1 & \iddots & \iddots & \iddots & \iddots \\
      1 & \iddots & \iddots & \iddots & \iddots \\
      1 & \iddots & \iddots & \iddots & \iddots \\
      1 & \iddots & \iddots & \iddots & \iddots \\
      1 & \iddots & \iddots & \iddots & \iddots \\
      1 & \iddots & \iddots & \iddots & \iddots \\
    \end{tabular}
    \end{center}

    Here, we multiply the corresponding terms to populate the table:

    \begin{center}
    \begin{tabular}[H]{c|cccc}
      & 0 & 1 & 1 & 1\\
      \hline
      0 & 0 & 0 & 0 & 0\\
      0 & 0 & 0 & 0 & 0\\
      0 & 0 & 0 & 0 & 0\\
      0 & 0 & 0 & 0 & 0\\
      0 & 0 & 0 & 0 & 0\\
      1 & 0 & 1 & 1 & 1 \\
      1 & 0 & 1 & 1 & 1 \\
      1 & 0 & 1 & 1 & 1 \\
      1 & 0 & 1 & 1 & 1 \\
      1 & 0 & 1 & 1 & 1 \\
      1 & 0 & 1 & 1 & 1 \\
    \end{tabular}
    \end{center}

    Now we add diagonals to find the product, which gives us:

    $$y[n]=\{ 0, (0+0), (0+0+0), (0+0+0+0), (0+0+0+0), $$
    $$(0+0+0+0), (0+0+1+0), (0+1+1+0), $$
    $$(0+1+1+1), (0+1+1+1), (0+1+1+1),(1+1+1), (1+1), 1 \}$$

    This can be simplifed to:

    $$y[n]=\left\{ 0, 0, 0, 0, 0, 0, 1, 2, 3, 3, 3, 3, 2, 1, 0\cdots\right\}$$

    Using the step function notation, we may write:

    $$y[n]=u[n-6]+u[n-7]+u[n-8]-u[n-12]-u[n-13]-u[n-14]$$

  \item

    We can use a method similar to question (4) to find $N$. Let us begin with a table:

    \begin{center}
      \begin{tabular}[H]{c|cccccc}
        & 1 & 1 & 1 & 1 & 1 & 1 & 1\\
        \hline
        1 & & & & & & & \\
        \vdots & & & & & & & \\
      \end{tabular}
    \end{center}

    Using the tabulating method, we know that, for there to be a value of $4$, $h[n]$ needs to exist for at least 4 different $n$. Therefore, let us begin with the minimum such value for $h[n]$, when $N=3$, which gives us the following table:

    \begin{center}
      \begin{tabular}[H]{c|cccccc}
        & 1 & 1 & 1 & 1 & 1 & 1 \\
        \hline
        1 & 1 & 1 & 1 & 1 & 1 & 1\\
        1 & 1 & 1 & 1 & 1 & 1 & 1\\
        1 & 1 & 1 & 1 & 1 & 1 & 1 \\
        1 & 1 & 1 & 1 & 1 & 1 & 1 \\
      \end{tabular}
    \end{center}

    This gives us $y[n]=\left\{  1, 2, 3, 4, 4, 4, 3, 2, 1, 0, \cdots\right\}$. With this result, we see that $y[3]=4$, and $y[9]=0$. Thus, we find that:

    $$\boxed{N=3}$$

  \item

    \begin{enumerate}

      \item We can express this as $x_1[n]=u[n-3]$

        Since this is an LTI system, we know that the output will be shifted by the same amount (shifting property), which gives us:

        $$\boxed{x_1[n]\to y_1[n]=\left( \frac{1}{4} \right)^{n-3}u[n-3]-\left( \frac{1}{4} \right)^{n-4}u[n-4]}$$

      \item This input can be expressed as: $x_2[n]=u[n]-u[n-4]$

        Once again by the shifting property, as well as by homogeneity and superposition, we can write:

        $$\boxed{x_2[n]\to y_2[n]=\left( \frac{1}{4} \right)^{n}u[n]-\left( \frac{1}{4} \right)^{n-1}u[n-1]-\left( \frac{1}{4} \right)^{n-4}u[n-4]+\left( \frac{1}{4} \right)^{n-5}u[n-5]}$$

      \item This input can be expressed as: $x_3[n]=2u[n]-2u[n-1]$

        By the shifting, homogenous, and superposition principles of LTI systems, we get:

        $$x_3[n]\to y_2[n]=2\left( \frac{1}{4} \right)^{n}u[n]-2\left( \frac{1}{4} \right)^{n-1}u[n-1]-2\left( \frac{1}{4} \right)^{n-1}u[n-1]+2\left( \frac{1}{4} \right)^{n-2}u[n-2]$$

        Which can be simplifed:

        $$\boxed{x_3[n]\to y_2[n]=2\left( \frac{1}{4} \right)^{n}u[n]-4\left( \frac{1}{4} \right)^{n-1}u[n-1]+2\left( \frac{1}{4} \right)^{n-2}u[n-2]}$$

    \end{enumerate}

  \item

    Per convolution properties, we know:

    $$x(t)*\delta(t-t_o)\Rightarrow x(t-t_o)$$

    Thus, looking at the input, in addition to the fact that this is an LTI system, we can write:

    $$\boxed{y(t)=x(t)*h(t)\to y(t)=x(t+2)-2x(t)}$$

    Plotting this shift, we get:

    \begin{figure}[H]
      \centering
      \include{Figures/HW3-7}
      \caption{Plot for $y(t)=x(t+2)-2x(t)$}
      \label{fig:2}
    \end{figure}

  \item

    \begin{enumerate}

      \item Using this, we can rewrite $x$ as:

        $$x(t)=u(t)-u(t-1)$$

        Which would make $h$:

        $$h(t)=u(t-2)-u(t-4)$$

        This gives us:

        $$y(t)=\int[u(t)-u(t-1)]*[u(t-2)-u(t-4)]\,dt$$

        Which expands to:

        $$y(t)=\int u(t)u(t-2)-u(t)u(t-4)-u(t-1)u(t-2)+u(t-1)u(t-4)\,dt$$

        To analyze, we can use the following properties:

        $$r(t)*r(t-T_1)=r(t-T_1)$$
        $$r(t-T_1)*r(t-T_2)=r(t-T_1-T_2)$$

        This gives us:

        $$y(t)=r(t-2)-r(t-4)-r(t-3)+r(t-5)$$
        $$\boxed{y(t)=r(t-2)-r(t-3)-r(t-4)+r(t-5)}$$

        And the plot becomes:

        \begin{figure}[H]
          \centering
          \include{Figures/HW3-8}
          \caption{Plot for $y(t)=r(t-2)-r(t-3)-r(t-4)+r(t-5)$}
          \label{fig:3}
        \end{figure}

      \item 

        We can determine $\frac{d}{dt}[y(t)]$ to be:

        $$\frac{d}{dt}[y(t)]=u(t-2)-u(t-3)-u(t-4)+u(t-5)$$

        The discontinuities may be identified by differentiating again to get:

        $$\frac{d^2}{dt^2}[y(t)]=\delta(t-2)-\delta(t-3)-\delta(t-4)+\delta(t-5)$$

        We know that each impulse represents a discontinuity; Therefore, we can tell that there are 4 discontinuities, at $t=2,3,4,$ and $5$, for $d/dt[y(t)]$

    \end{enumerate}

  \item

    \begin{enumerate}

      \item 

        We know that the impulse response can be determined if $x(t)=\delta(t)$:

        $$y(t)=\int_{-\infty}^{t}e^{-(t-\tau)}x(\tau-2)\,d\tau$$
        $$y(t)=\int_{-\infty}^{t}e^{-(t-\tau)}\delta(\tau-2)\,d\tau$$

        We also know from the property of the impulse that:

        $$\int_{-\infty}^{\infty} x(t)\delta(t-t_o)\,dt=x(t_o)$$

        Thus, we can see that:

        $$\boxed{h(t)=e^{-(t-2)}}$$

      \item 

        We may begin by writing $x(t)$:

        $$x(t)=u(t+1)-u(t-2)$$

        Alternatively, this may be written in laplace form as:

        $$x(s)=\frac{e^s}{s}-\frac{e^{-2s}}{s+1}$$

        Which gives us:

        $$h(s)=\frac{1}{s+1}$$

        Multiplying the two togetherm, we get:

        $$x(s)h(s)=e^s\left[ \frac{1}{s}-\frac{1}{s+1} \right]-\frac{e^{-2s}}{(s+1)^2}$$

        We then take the inverse laplace transform to finally find:

        $$\boxed{y(t)=u(t+1)-e^{-t-1}u(t+1)-(t-2)e^{2-t}u(t-2)}$$

        $$$$

    \end{enumerate}

\end{enumerate}

\end{document}

