%%%%%%%%%%%%%%%%%%%%%%%%%%%%%%%%%%%%%%%%%%%%%%%%%%%%%%%%%%%%%%%%%%%%%%%%%%%%%%%%%%%%%%%%%%%%%%%%%%%%%%%%%%%%%%%%%%%%%%%%%%%%%%%%%%%%%%%%%%%%%%%%%%%%%%%%%%%%%%%%%%%
% Written By Michael Brodskiy
% Class: Fundamentals of Linear Systems
% Professor: I. Salama
%%%%%%%%%%%%%%%%%%%%%%%%%%%%%%%%%%%%%%%%%%%%%%%%%%%%%%%%%%%%%%%%%%%%%%%%%%%%%%%%%%%%%%%%%%%%%%%%%%%%%%%%%%%%%%%%%%%%%%%%%%%%%%%%%%%%%%%%%%%%%%%%%%%%%%%%%%%%%%%%%%%

\include{Includes.tex}

\title{Homework 5}
\date{\today}
\author{Michael Brodskiy\\ \small Professor: I. Salama}

\begin{document}

\maketitle

\begin{enumerate}

  \item

    \begin{enumerate}

      \item 

        We may begin by rewriting $S_2$ as:

        $$w[n]=y[n]-\frac{1}{2}y[n-1]$$

        $S_1$ may be rewritten in a similar format to get:

        $$x[n]=w[n]-\frac{1}{4}w[n-1]$$

        Substituting the first equation into the second, we get:

        $$x[n]=y[n]-\frac{1}{2}y[n-1]-\frac{1}{4}\left[ y[n-1]-\frac{1}{2}y[n-2] \right]$$

        This can be simplified to:

        $$\boxed{x[n]=y[n]-\frac{3}{4}y[n-1]+\frac{1}{8}y[n-2]}$$

      \item 

        We may find the impulse response by taking $x[n]\to\delta[n]$. This gives us:

        $$w[n]=\frac{1}{4}w[n-1]+\delta[n]$$

        Taking the $z$ transform, we may write:

        $$W(z)=\frac{1}{\left( 1-\frac{1}{4}z^{-1} \right)},\quad |z|>.25$$
        $$W(z)=\frac{z}{\left( z-\frac{1}{4} \right)},\quad |z|>.25$$
        $$\boxed{w[n]=\left( \frac{1}{4} \right)^{n}u[n]}$$

        Finding the individual impulse response for $S_2$, we get:

        $$Y(z)=\frac{1}{1-\frac{1}{2}z^{-1}},\quad |z|>.5$$
        $$Y(z)=\frac{z}{z-\frac{1}{2}},\quad |z|>.5$$
        $$\boxed{y[n]=\left( \frac{1}{2} \right)^nu[n]}$$

      \item 

        We can once again use the $z$ transform, this time using the equation obtained in (a), to get:

        $$Y(z)=\frac{1}{1-\frac{3}{4}z^{-1}+\frac{1}{8}z^{-2}}$$
        $$Y(z)=\frac{z^2}{z^2-\frac{3}{4}z+\frac{1}{8}}$$
        $$Y(z)=\frac{z^2}{\left( z-\frac{1}{2} \right)\left( z-\frac{1}{4} \right)},\quad |z|>.5$$

        We can use partial fraction decomposition, by rearranging:

        $$\frac{Y(z)}{z}=\frac{z}{\left( z-\frac{1}{2} \right)\left( z-\frac{1}{4} \right)},\quad |z|>.5$$
        $$\frac{Y(z)}{z}=\frac{A}{z-.25}+\frac{B}{z-.5}$$

        We may find: $A=-1$, $B=2$, which gives us:

        $$Y(z)=\frac{-z}{z-.25}+\frac{2z}{z-.5},\quad |z|>.5$$

        We take the inverse transform to get:

        $$\boxed{y[n]=2\left( \frac{1}{2} \right)^nu[n]-\left(\frac{1}{4}\right)u[n]}$$

    \end{enumerate}

  \item

    \begin{enumerate}

      \item 

        This gives us:

        $$A\left( \frac{1}{4} \right)^{n}-\frac{A}{4}\left( \frac{1}{4} \right)^{n-1}=0$$
        $$A\left( \frac{1}{4} \right)^{n}-A\left( \frac{1}{4} \right)^{n}=0$$

        The \underline{two terms and subtract, and do equal zero} \textcolor{green}{\checkmark}

      \item 

        We may begin by substituting:

        $$B\left( \frac{1}{2} \right)^{n}-\frac{B}{4}\left( \frac{1}{2} \right)^{n-1}=\left( \frac{1}{2} \right)^n$$

        We subtract over:
        
        $$\frac{B}{4}\left( \frac{1}{2} \right)^{n-1}=B\left( \frac{1}{2} \right)^{n}-\left( \frac{1}{2} \right)^n$$

        From this, we can set up an expression for $B$:

        $$\frac{B}{4}=\frac{1}{2}\left( B-1 \right)$$

        And now we solve:

        $$-\frac{B}{4}= -\frac{1}{2}$$
        $$\boxed{B= 2}$$

      \item 

        We first work to find the value of $y[0]$:

        $$y[0]-\frac{1}{4}y[-1]=\left( \frac{1}{2} \right)^{0}$$

        We know the term that occurs before $n=0$ is zero due to the rest condition, and, thus:

        $$y[0]=1$$

        Now we plug this into the overall solution:

        $$y[0]=A\left( \frac{1}{4} \right)^0+2\left( \frac{1}{2} \right)^0$$
        $$A+2=1$$
        $$\boxed{A=-1}$$

        Thus, we see that the solution is:

        $$y[n]=-\left( \frac{1}{4} \right)^n+2\left( \frac{1}{2} \right)^n$$

        Which can be simplified:

        $$\boxed{y[n]=\left( \frac{1}{2} \right)^{n-1}-\left( \frac{1}{4} \right)^n}$$

    \end{enumerate}

  \item

    \begin{enumerate}

      \item 

        Setting up the Laplace Transform, we get:

        $$X(s)=\int_{2}^{\infty}e^{-(4+s)t}\,dt$$
        $$X(s)=-\frac{e^{-(4+s)t}}{4+s}\Big|_2^{\infty}$$
        $$X(s)=\frac{e^{-2(4+s)}}{s+4}$$
        $$\boxed{X(s)=\frac{e^{-2s-8}}{s+4}}$$

        Since the equation is right-sided, the ROC is to the right of the right-most pole; there is one pole at $s=-4$, so the ROC is $\text{Re}\left\{ s \right\}>-4\longrightarrow \sigma >-4$ (since $s=\sigma+j\omega$)

      \item 

        We may find the Laplace Transform to be:

        $$G(s)=\int_{-\infty}^{-2} Ae^{-(4+s)t}\,dt$$
        $$G(s)=-A\frac{e^{-(4+s)t}}{4+s}\Big|_{-\infty}^{-2}$$
        $$G(s)=-\frac{A}{4+s}\left[e^{2(4+s)}-e^{\infty(4+s)}\right]$$

        We may see that $G(s)$ converge only when $s$ reaches the ROC at $\sigma<-4$

        We can thus drop the term to get

        $$G(s)=-\frac{Ae^{2s+8}}{4+s}$$

        We can check the value of $A$:

        $$-Ae^{2s+8}=e^{-2s-8}$$

        We may see that, though the exponents will never be the same, we may take $A=-1$ to create a similar algebraic form. Thus, we say:

        $$\boxed{A=-1}$$

    \end{enumerate}

  \item

    \begin{enumerate}

      \item We may calculate the Laplace transform for the time-shifted signal as:

        $$X_1(s)=\int_{-\infty}^{\infty}x(t-t_o)e^{-st}\,dt$$

        Taking $t-t_o= n$, we write:

        $$X_1(s)=\int_{-\infty}^{\infty}x(n)e^{-s(n+t_o)}\,dn$$
        $$X_1(s)=e^{-st_o}\underbrace{\int_{-\infty}^{\infty}x(n)e^{-sn}\,dn}_{X(s)}$$

        Which gives us:

        $$\boxed{X_1(s)=e^{-st_o}X(s)}$$

        And we may see that the ROC remains to be $R$.

      \item We may express the signal as:

        $$y(t)=u(t)-2u(t-2)+u(t-4)$$

        Thus, we use our table of known transforms to get:

        $$\boxed{Y(s)=\frac{1}{s}-\frac{2e^{-2t}}{s}+\frac{e^{-4t}}{s}}$$

        We may see that the ROC is: $\boxed{\sigma>0}$

    \end{enumerate}

  \item

    We may rewrite $x(t)$ as:

    $$x(t)=e^t\sin(5t)u(-t)$$

    Which gives us:

    $$X(s)=\int_{-\infty}^{0}e^{-(s-1)t}\sin(5t)\,dt$$
    $$X(s)=-\frac{5}{(s-1)^2+25}$$
    $$\boxed{X(s)=-\frac{5}{s^2-2s+26}}$$

    We may see by the second equation that the region of convergence is left-handed, and occurs at $\boxed{\text{ROC: }\text{Re}\left\{s\right\}-1<0\longrightarrow \sigma <1}$. The poles will occur at the solutions to the quadratic in the denominator:

    $$s^2-2s+26=0$$
    $$\frac{2\pm\sqrt{4-4(1)(26)}}{2}$$
    $$\frac{2\pm10j}{2}$$
    $$\boxed{\text{Poles at: }s=1\pm 5j}$$

  \item

    Using partial fraction decomposition, we may write:

    $$\frac{s-1}{(s+1)(s+3)(s^2+4s+20)}=\frac{A}{s+1}+\frac{B}{s+3}+\frac{Cs+D}{s^2+4s+20}$$

    And then:

    $$(s+3)(s^2+4s+20)A+(s+1)(s^2+4s+20)B+(s+1)(s+3)(Cs+D)=s-1$$
    $$As^3+7As^2+32As+60A+Bs^3+5Bs^2+24Bs+20B+Cs^3+4Cs^2+3Cs+Ds^2+4Ds+3D=s-1$$

    From this, we may derive:

    $$A+B+C=0$$
    $$7A+5B+4C+D=0$$
    $$32A+24B+3C+4D=1$$
    $$60A+20B+3D=-1$$

    Using a solver, we obtain:

    $$\left\{\begin{array}{lll} A&=& -\frac{1}{17}\\B&=&\frac{2}{17} \\C&=&-\frac{1}{17} \\D&=&\frac{1}{17} \end{array}$$

      Now with our coefficients, we take the inverse Laplace transforms to get:

      $$x(t)=-\frac{1}{17}\mathcal{L}^{-1}\left\{ \frac{1}{s+1} \right\}+\frac{2}{17}\mathcal{L}^{-1}\left\{ \frac{1}{s+3} \right\}-\frac{1}{17}\mathcal{L}^{-1}\left\{ \frac{(s+2)}{(s+2)^2+4^2} \right\}+\frac{1}{17}\mathcal{L}^{-1}\left\{ \frac{4}{(s+2)^2+4^2} \right\}$$

      And finally, we get:

      $$\boxed{x(t)=-\frac{e^{-t}}{17}+\frac{2e^{-3t}}{17}-\frac{e^{-2t}\cos(4t)}{17}+\frac{e^{-2t}\sin(4t)}{17}}$$

      For each term, in order, the ROCs may be identified as: $\sigma=-1$, $\sigma=-3$, and $\sigma=-4$. Since all of the signals are causal, we know the ROCs are to the right. Thus, there will be overlap when $\sigma$ is greater than the greatest individual ROC, or $\sigma=-1$. This makes the combined ROC: $\boxed{\sigma > -1}$

      We may observe that \underline{four individual signals} contribute to the Laplace Transform. Furthermore, we can find the zeroes and poles as:

      $$\boxed{\text{Zero: }s-1=0\to s=1}$$
      $$\boxed{\text{Poles: }\left\{\begin{array}{lll} s+1&=&0\\s+3&=&0\\(s^2+4s+20)&=&0\end{array}\to\left\{\begin{array}{lll} s&=&-1\\s&=&-3\\s&=&-2\pm4j\end{array}}$$

          This can be plotted as:

          \begin{figure}[H]
            \centering
            \include{Figures/HW5-6}
            \caption{Pole-Zero Plot of $X(s)$}
            \label{fig:1}
          \end{figure}

  \item

    \begin{enumerate}

      \item 

        Per the basic Laplace transformation tables, we may write:

        $$\boxed{X(s)=\frac{1}{s+2}-\frac{1}{s-4}}$$

        We may observe that there are two ROCs, $\sigma<4$ and $\sigma>-2$, which gives us overlap in the region:

        $$\boxed{-2<\sigma<4}$$

        This gives us the following plot:

        \begin{figure}[H]
          \centering
          \include{Figures/HW5-7a}
          \caption{Pole-Zero Plot for 7(a)}
          \label{fig:2}
        \end{figure}

      \item 

        Once again employing the tables, we find:

        $$X(s)=\frac{1}{s+3}+\frac{4}{(s+2)^2+16}$$

        Rearranging to simplify ROC analysis, we get:

        $$\boxed{X(s)=\frac{s^2+8s+32}{(s+3)(s^2+4s+20)}}$$

        From this, we can determine that the zeros are at $s=-4\pm4j$ and there are poles at $-3$ and $-4\pm4j$. Since both are right-sided, we may notice that the ROC occurs to the right of the greatest pole, or $\sigma>-3$

        \begin{figure}[H]
          \centering
          \include{Figures/HW5-7b}
          \caption{Pole-Zero Plot for 7(b)}
          \label{fig:3}
        \end{figure}

      \item 

        We may rewrite $x(t)$ as:

        $$x(t)=-te^{2t}u(-t)+te^{-2t}u(t)$$

        Using our known transforms:

        $$X(s)=-\left[ -\frac{d}{ds}\left( \frac{1}{s-2} \right) \right]-\frac{d}{ds}\left( \frac{1}{s+2} \right)$$
        $$\boxed{X(s)=\frac{1}{(s+2)^2}-\frac{1}{(s-2)^2}}$$

        To simplify analysis, we rearrange to get:

        $$X(s)=\frac{(s-2)^2-(s+2)^2}{(s+2)^2(s-2)^2}$$
        $$X(s)=\frac{-8s}{(s+2)^2(s-2)^2}$$

        From this, we observe that there is a zero at $s=0$, and there are poles (both of order 2) $\sigma=\pm 2$. Since both signals are right-handed, the ROC is in: $\sigma>2$. This gives us the following plot:

        \begin{figure}[H]
          \centering
          \include{Figures/HW5-7c}
          \caption{Pole-Zero Plot for 7(c)}
          \label{fig:4}
        \end{figure}

      \item 

        We may begin by writing:

        $$x(t)=3r(t)-3r(t-1))-3u(t-2)$$

        This gives us the transform as:

        $$\boxed{X(s)=\frac{3}{s^2}-\frac{3}{s^2}e^{s}-\frac{3}{s}e^{2s}}$$

        We may observe that there are no zeros, but there is a pole at $s=0$, which gives an ROC of $s>0$ and the following plot:

        \begin{figure}[H]
          \centering
          \include{Figures/HW5-7d}
          \caption{Pole-Zero Plot for 7(d)}
          \label{fig:5}
        \end{figure}

    \end{enumerate}

  \item Since the function is absolutely integrable, we know that it is bounded by BIBO stability. This means that the ROC contains the $j \omega$ axis, and that the ROC does not have any poles. Knowing this, we can deduce:

    \begin{enumerate}

      \item \underline{The function can not be finite}

        This is due to the fact that, since there is a pole at $s=-4$, we know that the signal contains $x(t)=e^{-4t}$. Since this function extends to $t\to\infty$, we know that the signal can not be finite. Also, note that a finite signal, by definition, does not contain poles.

      \item \underline{The function can not be left-sided}

        Since we know that, due to being absolutely integrable, the function must contain the $j \omega$ axis, the right-most pole must be to the right of this axis. Since $s=-4$ is to the left of the axis, the signal can not be left-sided.

      \item \underline{The function can be right-sided}

        An example of such a signal would be:

        $$\boxed{x(t)=e^{-4t}u(t)}$$

      \item \underline{The function can be two-sided} (given that there may be multiple poles â€” the problem states that there \textit{is} a pole at $s=-4$, but does not state that it is the only pole)

        Take, for example, the signal (where $n>0$):

        $$x(t)=e^{-4t}u(t)+e^{nt}u(-t)$$

        This signal is two-sided, contains $s=-4$ as a pole, is absolutely integrable (and thus contains the $j\omega$ axis), which makes it a valid signal.

      \item 

        \begin{itemize}

          \item With the absolutely integrable rule change from $x(t)$ to $x(t)e^{-2t}$, nothing would change. This is because it would mean that, instead of the $j\omega$ axis, the ROC would now need to contain the $\sigma=2$ axis. Thus, the properties remain the same since this is to the right of the pole at $s=-4$.

          \item Changing the condition such that $x(t)e^{5t}$ is absolutely integrable would change things. This would mean that the ROC would need to contain the $\sigma=-5$ axis, instead of the $j\omega$ axis, which is left of the pole. Thus, the signal \underline{can now be left-sided, but not right-sided}

        \end{itemize}

      \item 

        We know that, due to the integrable rule, the ROC must be right of the right-most pole (to contain the $j\omega$ axis). This means that the ROC is $\sigma>-2$. From here, we write $X(s)$ as:

        $$X(s)=\frac{N(s-1)}{(s+4)(s+2-j2)}$$

        We can solve for $N$ by using the initial condition:

        $$X(0)=\frac{-N}{4(2-j2)}$$
        $$\frac{-N}{4(2-j2)}=-1$$
        $$N=8-j8$$

        This gives us:

        $$\boxed{X(s)=\frac{(8-j8)(s-1)}{(s+4)(s+2-j2)}}$$

    \end{enumerate}

  \item

    \begin{enumerate}

      \item Using the table, we get:

        $$\boxed{x(t)=\frac{1}{3}\sin(3t)u(t)}$$

        And we see that the ROC is $\boxed{\sigma>0}$

      \item Using the table, we get:

        $$\boxed{x(t)=-\cos(2t)u(-t)}$$

        And we see that the ROC is $\boxed{\sigma<0}$

      \item Using the table, we get:

        $$\boxed{x(t)=-e^{-5t}\cos(4t)u(-t)}$$

        And we see that the ROC is $\boxed{\sigma<-5}$

      \item To simplify analysis, we may rewrite this as:

        $$X(s)=\frac{1}{(s+4)(s+2)}$$

        We use partial fraction decomposition to get:

        $$X(s)=\frac{A}{s+2}+\frac{B}{s+4}$$

        Solving, we find: $A=-.5$ and $B=.5$, which gives us:

        $$X(s)=\frac{.5}{s+4}-\frac{.5}{s+2}$$

        Finally, using the table, we get:

        $$\boxed{x(t)=-\frac{1}{2}\left[ e^{-4t}u(t)+e^{-2t}u(-t) \right]}$$

        And we see the ROC is: $\boxed{-4<\sigma<-2}$

      \item This can be expanded to:

        $$X(s)=\frac{(s+2)^2-5s-10+8}{(s+2)^2}$$

        We then break this into:

        $$X(s)=1-\frac{5}{s+2}+\frac{8}{(s+2)^2}$$

        We now use the table to find:

        $$\boxed{x(t)=\delta(t)-5e^{-2t}u(t)+8te^{-2t}u(t)}$$

        With ROC: $\boxed{\sigma>-2}$

    \end{enumerate}

\end{enumerate}

\end{document}

