%%%%%%%%%%%%%%%%%%%%%%%%%%%%%%%%%%%%%%%%%%%%%%%%%%%%%%%%%%%%%%%%%%%%%%%%%%%%%%%%%%%%%%%%%%%%%%%%%%%%%%%%%%%%%%%%%%%%%%%%%%%%%%%%%%%%%%%%%%%%%%%%%%%%%%%%%%%%%%%%%%%
% Written By Michael Brodskiy
% Class: Fundamentals of Linear Systems
% Professor: I. Salama
%%%%%%%%%%%%%%%%%%%%%%%%%%%%%%%%%%%%%%%%%%%%%%%%%%%%%%%%%%%%%%%%%%%%%%%%%%%%%%%%%%%%%%%%%%%%%%%%%%%%%%%%%%%%%%%%%%%%%%%%%%%%%%%%%%%%%%%%%%%%%%%%%%%%%%%%%%%%%%%%%%%

\include{Includes.tex}

\title{Quiz 3}
\date{\today}
\author{Michael Brodskiy\\ \small Professor: I. Salama}

\begin{document}

\maketitle

\begin{enumerate}[label=\Alph*.]

  \item Taking the Laplace transform of the transfer function, we get:

    $$s^2Y(s)+2sY(s)-8Y(s)=sX(s)+3X(s)$$

    Given that the transfer function may be expressed as:

    $$H(s)=\frac{Y(s)}{X(s)}$$

    We rearrange to get:

    $$[s^2+2s-8]Y(s)=[s+3]X(s)$$

    This gives us:

    $$\boxed{H(s)=\frac{s+3}{s^2+2s-8}}$$

  \item Given that the function is stable, we know that the ROC must contain the $j\omega$ axis. Since we see that the poles are at $s=2,-4$, we know that the ROC can be expressed as the real values in between the two poles (double-sided):

    $$\boxed{\text{R.O.C: }-4<\sigma<2}$$

  \item We see that there are poles at $\sigma=2,-4$ and a zero at $\sigma=-3$. This gives us:

    \begin{figure}[H]
      \centering
      \include{Figures/Q3C}
      \caption{Pole-Zero Plot of $H(s)$}
      \label{fig:1}
    \end{figure}

  \item The system has one zero located at $\sigma=-3$.

  \item Since the signal is double-sided, we know it \underline{is not} causal.

  \item We may begin by using partial fractions to obtain an equivalent $H(s)$. This gives us:

    $$\frac{s+3}{(s+4)(s-2)}=\frac{A}{s+4}+\frac{B}{s-2}$$

    Using partial fraction decomposition, we get $A=1/6$ and $B=5/6$:

    $$H(s)=\frac{1/6}{s+4}+\frac{5/6}{s-2}$$

    Taking the inverse transform, we get:

    $$\boxed{h(t)=\frac{5}{6}e^{2t}u(-t)+\frac{1}{6}e^{-4t}u(t)}$$

  \item

    \begin{enumerate}[label=\Roman*.]

      \item Using our transform tables, the transform of this input is:

        $$\boxed{X(s)=\frac{6}{s+3}}$$

        Since the signal is right-handed, the R.O.C is:

        $$\boxed{\text{R.O.C: } \sigma>-3}$$

      \item We determine the output by multiplying together the response and input. This gives us:

        $$Y(s)=\left( \frac{s+3}{(s-2)(s+4)} \right)\left( \frac{6}{s+3} \right)$$
        $$\boxed{Y(s)=\frac{6}{(s-2)(s+4)}}$$

        We combine the two regions of convergence, which means the R.O.C is:

        $$\boxed{\text{R.O.C: }-3<\sigma<2}$$

      \item We use partial fractions to get:

        $$Y(s)=\frac{1}{s+4}+\frac{3}{s-2}$$

        Taking the inverse transform, we get:

        $$\boxed{y(t)=e^{-4t}u(t)+3e^{2t}u(-t)}$$

    \end{enumerate}

\end{enumerate}

\end{document}

